compcert/common/Values.v
@@ -150,21 +150,76 @@ Proof.
   auto.
 Defined.
 
-Definition has_rettype (v: val) (r: rettype) : Prop :=
+(** Strict matching between values and extended types:
+    the value cannot be [Vundef], unless the type is [Tvoid].
+    This matching is used to characterize arguments to function calls. *)
+
+Definition has_argtype (v: val) (x: xtype) : Prop :=
+  match x, v with
+  | Xbool, Vint n => n = Int.zero \/ n = Int.one
+  | Xint8signed, Vint n => n = Int.sign_ext 8 n
+  | Xint8unsigned, Vint n => n = Int.zero_ext 8 n
+  | Xint16signed, Vint n => n = Int.sign_ext 16 n
+  | Xint16unsigned, Vint n => n = Int.zero_ext 16 n
+  | Xint, Vint _ => True
+  | Xint, Vptr _ _ => Archi.ptr64 = false
+  | Xlong, Vlong _ => True
+  | Xlong, Vptr _ _ => Archi.ptr64 = true
+  | Xfloat, Vfloat _ => True
+  | Xsingle, Vsingle _ => True
+  | Xptr, Vptr _ _ => True
+  | Xptr, Vint _ => Archi.ptr64 = false
+  | Xptr, Vlong _ => Archi.ptr64 = true
+  | Xany32, (Vint _ | Vsingle _) => True
+  | Xany32, Vptr _ _ => Archi.ptr64 = false
+  | Xany64, (Vint _ | Vlong _ | Vptr _ _ | Vsingle _ | Vfloat _) => True
+  | Xvoid, _ => True
+  | _, _ => False
+  end.
+
+Definition has_argtype_list : list val -> list xtype -> Prop := list_forall2 has_argtype.
+
+(** Lax matching between values and extended types:
+    [Vundef] belongs to every type.
+    This matching is used to characterize return values from external calls
+    and built-in functions. *)
+
+Definition has_rettype (v: val) (r: xtype) : Prop :=
   match r, v with
-  | Tret t, _ => has_type v t
-  | Tint8signed, Vint n => n = Int.sign_ext 8 n
-  | Tint8unsigned, Vint n => n = Int.zero_ext 8 n
-  | Tint16signed, Vint n => n = Int.sign_ext 16 n
-  | Tint16unsigned, Vint n => n = Int.zero_ext 16 n
+  | Xbool, Vint n => n = Int.zero \/ n = Int.one
+  | Xint8signed, Vint n => n = Int.sign_ext 8 n
+  | Xint8unsigned, Vint n => n = Int.zero_ext 8 n
+  | Xint16signed, Vint n => n = Int.sign_ext 16 n
+  | Xint16unsigned, Vint n => n = Int.zero_ext 16 n
+  | Xint, Vint _ => True
+  | Xint, Vptr _ _ => Archi.ptr64 = false
+  | Xlong, Vlong _ => True
+  | Xlong, Vptr _ _ => Archi.ptr64 = true
+  | Xfloat, Vfloat _ => True
+  | Xsingle, Vsingle _ => True
+  | Xptr, Vptr _ _ => True
+  | Xptr, Vint _ => Archi.ptr64 = false
+  | Xptr, Vlong _ => Archi.ptr64 = true
+  | Xany32, (Vint _ | Vsingle _) => True
+  | Xany32, Vptr _ _ => Archi.ptr64 = false
+  | Xany64, _ => True
   | _, Vundef => True
   | _, _ => False
   end.
 
-Lemma has_proj_rettype: forall v r,
-  has_rettype v r -> has_type v (proj_rettype r).
+Lemma has_proj_xtype: forall v t,
+  has_rettype v t -> has_type v (proj_xtype t).
 Proof.
-  destruct r; simpl; intros; auto; destruct v; try contradiction; exact I.
+  intros. destruct t, v; simpl in *; auto; try contradiction.
+- unfold Tptr; rewrite H; auto.
+- unfold Tptr; rewrite H; auto.
+- unfold Tptr; destruct Archi.ptr64; auto.
+Qed.
+
+Lemma has_inj_type: forall v t,
+  has_type v t -> has_rettype v (inj_type t).
+Proof.
+  intros. destruct v, t; simpl in *; auto.
 Qed.
 
 (** Truth values.  Non-zero integers are treated as [True].
@@ -271,6 +326,10 @@ Definition notint (v: val) : val :=
   end.
 
 Definition of_bool (b: bool): val := if b then Vtrue else Vfalse.
+
+Definition is_bool (v: val) : bool := eq v Vtrue || eq v Vfalse.
+
+Definition norm_bool (v: val) : val := if is_bool v then v else Vundef.
 
 Definition boolval (v: val) : val :=
   match v with
@@ -1005,6 +1064,7 @@ Definition select (cmp: option bool) (v1 v2: val) (ty: typ) :=
 
 Definition load_result (chunk: memory_chunk) (v: val) :=
   match chunk, v with
+  | Mbool, Vint n => norm_bool (Vint (Int.zero_ext 8 n))
   | Mint8signed, Vint n => Vint (Int.sign_ext 8 n)
   | Mint8unsigned, Vint n => Vint (Int.zero_ext 8 n)
   | Mint16signed, Vint n => Vint (Int.sign_ext 16 n)
@@ -1021,10 +1081,18 @@ Definition load_result (chunk: memory_chunk) (v: val) :=
   | _, _ => Vundef
   end.
 
-Lemma load_result_rettype:
-  forall chunk v, has_rettype (load_result chunk v) (rettype_of_chunk chunk).
+Lemma norm_bool_cases:
+  forall v, norm_bool v = Vundef \/ norm_bool v = Vfalse \/ norm_bool v = Vtrue.
+Proof.
+  intros. unfold norm_bool, is_bool.
+  destruct (eq v Vtrue); auto. destruct (eq v Vfalse); auto.
+Qed.
+
+Lemma load_result_xtype:
+  forall chunk v, has_rettype (load_result chunk v) (xtype_of_chunk chunk).
 Proof.
   intros. unfold has_rettype; destruct chunk; destruct v; simpl; auto.
+- destruct (norm_bool_cases (Vint (Int.zero_ext 8 i))) as [A | [A | A]]; rewrite A; simpl; auto.
 - rewrite Int.sign_ext_idem by lia; auto.
 - rewrite Int.zero_ext_idem by lia; auto.
 - rewrite Int.sign_ext_idem by lia; auto.
@@ -1037,8 +1105,8 @@ Qed.
 Lemma load_result_type:
   forall chunk v, has_type (load_result chunk v) (type_of_chunk chunk).
 Proof.
-  intros. rewrite <- proj_rettype_of_chunk. apply has_proj_rettype.
-  apply load_result_rettype.
+  intros. rewrite <-proj_xtype_of_chunk. apply has_proj_xtype.
+  apply load_result_xtype.
 Qed.
 
 Lemma load_result_same:
@@ -1076,6 +1144,18 @@ Proof.
   intros. destruct ob; simpl in H.
   destruct b0; simpl in H; inv H; auto.
   inv H.
+Qed.
+
+Theorem of_bool_is_bool:
+  forall b, is_bool (of_bool b) = true.
+Proof.
+  destruct b; reflexivity.
+Qed.
+
+Theorem norm_bool_idem:
+  forall v, norm_bool (norm_bool v) = norm_bool v.
+Proof.
+  intros; unfold norm_bool. destruct (is_bool v) eqn:E; auto. rewrite E; auto.
 Qed.
 
 Theorem notbool_negb_1:
@@ -2027,6 +2107,18 @@ Proof.
   intros. inv H. auto. destruct chunk; simpl; auto.
 Qed.
 
+Lemma norm_bool_is_lessdef:
+  forall v, lessdef (norm_bool v) v.
+Proof.
+  intros; unfold norm_bool. destruct is_bool; auto.
+Qed.
+
+Lemma norm_bool_lessdef:
+  forall v1 v2, lessdef v1 v2 -> lessdef (norm_bool v1) (norm_bool v2).
+Proof.
+  intros; inv H; auto.
+Qed.
+
 Lemma zero_ext_lessdef:
   forall n v1 v2, lessdef v1 v2 -> lessdef (zero_ext n v1) (zero_ext n v2).
 Proof.
@@ -2192,6 +2284,20 @@ Proof.
   apply normalize_lessdef. destruct b; auto.
 Qed.
 
+Lemma has_argtype_lessdef: forall v r v',
+  has_argtype v r -> lessdef v v' -> has_argtype v' r.
+Proof.
+  intros. inv H0; auto. destruct r; elim H || exact I.
+Qed.
+
+Lemma has_argtype_list_lessdef: forall vl rl vl',
+  has_argtype_list vl rl -> lessdef_list vl vl' -> has_argtype_list vl' rl.
+Proof.
+  unfold has_argtype_list; intros. revert vl vl' H0 rl H. induction 1; intros.
+- inv H. constructor.
+- inv H1. constructor; eauto using has_argtype_lessdef.
+Qed.
+
 (** * Values and memory injections *)
 
 (** A memory injection [f] is a function from addresses to either [None]
@@ -2254,7 +2360,9 @@ Lemma load_result_inject:
   inject f v1 v2 ->
   inject f (Val.load_result chunk v1) (Val.load_result chunk v2).
 Proof.
-  intros. inv H; destruct chunk; simpl; try constructor; destruct Archi.ptr64; econstructor; eauto.
+  intros. unfold Val.load_result.
+  inv H; destruct chunk; try constructor; try (destruct Archi.ptr64; econstructor; now eauto).
+  unfold norm_bool. destruct is_bool; auto.
 Qed.
 
 Remark add_inject:
@@ -2504,6 +2612,20 @@ Proof.
 - subst ob; auto.
 - subst ob'; destruct ob as [b|]; auto.
   apply normalize_inject. destruct b; auto.
+Qed.
+
+Lemma has_argtype_inject: forall v r v',
+  has_argtype v r -> inject f v v' -> has_argtype v' r.
+Proof.
+  intros. inv H0; destruct r; try contradiction; auto.
+Qed.
+
+Lemma has_argtype_list_inject: forall vl rl vl',
+  has_argtype_list vl rl -> inject_list f vl vl' -> has_argtype_list vl' rl.
+Proof.
+  unfold has_argtype_list; intros. revert vl vl' H0 rl H. induction 1; intros.
+- inv H. constructor.
+- inv H1. constructor; eauto using has_argtype_inject.
 Qed.
 
 End VAL_INJ_OPS.
