floyd/replace_refill_reptype_lemmas.v
@@ -189,7 +189,7 @@ Ltac cbv_proj_struct H :=
      ident_eq peq Pos.eq_dec BinNums.positive_rec positive_rect
     sumbool_rec sumbool_rect bool_dec bool_rec bool_rect option_rec option_rect
     eq_rect_r eq_rect eq_rec_r eq_rec eq_sym eq_trans f_equal
-    type_eq type_rec type_rect typelist_eq typelist_rec typelist_rect
+    type_eq type_rec type_rect
     intsize_rec intsize_rect signedness_rec signedness_rect floatsize_rec floatsize_rect
     tvoid tschar tuchar tshort tushort tint
     tuint tbool tlong tulong tfloat tdouble tptr tarray noattr
