progs64/logical_compare.v
@@ -6,7 +6,7 @@ Local Open Scope string_scope.
 Local Open Scope clight_scope.
 
 Module Info.
-  Definition version := "3.12".
+  Definition version := "3.15".
   Definition build_number := "".
   Definition build_tag := "".
   Definition build_branch := "".
@@ -19,67 +19,160 @@ Module Info.
   Definition normalized := true.
 End Info.
 
-Definition ___builtin_annot : ident := 17%positive.
-Definition ___builtin_annot_intval : ident := 18%positive.
-Definition ___builtin_bswap : ident := 2%positive.
-Definition ___builtin_bswap16 : ident := 4%positive.
-Definition ___builtin_bswap32 : ident := 3%positive.
-Definition ___builtin_bswap64 : ident := 1%positive.
-Definition ___builtin_clz : ident := 5%positive.
-Definition ___builtin_clzl : ident := 6%positive.
-Definition ___builtin_clzll : ident := 7%positive.
-Definition ___builtin_ctz : ident := 8%positive.
-Definition ___builtin_ctzl : ident := 9%positive.
-Definition ___builtin_ctzll : ident := 10%positive.
-Definition ___builtin_debug : ident := 36%positive.
-Definition ___builtin_expect : ident := 25%positive.
-Definition ___builtin_fabs : ident := 11%positive.
-Definition ___builtin_fabsf : ident := 12%positive.
-Definition ___builtin_fmadd : ident := 28%positive.
-Definition ___builtin_fmax : ident := 26%positive.
-Definition ___builtin_fmin : ident := 27%positive.
-Definition ___builtin_fmsub : ident := 29%positive.
-Definition ___builtin_fnmadd : ident := 30%positive.
-Definition ___builtin_fnmsub : ident := 31%positive.
-Definition ___builtin_fsqrt : ident := 13%positive.
-Definition ___builtin_membar : ident := 19%positive.
-Definition ___builtin_memcpy_aligned : ident := 15%positive.
-Definition ___builtin_read16_reversed : ident := 32%positive.
-Definition ___builtin_read32_reversed : ident := 33%positive.
-Definition ___builtin_sel : ident := 16%positive.
-Definition ___builtin_sqrt : ident := 14%positive.
-Definition ___builtin_unreachable : ident := 24%positive.
-Definition ___builtin_va_arg : ident := 21%positive.
-Definition ___builtin_va_copy : ident := 22%positive.
-Definition ___builtin_va_end : ident := 23%positive.
-Definition ___builtin_va_start : ident := 20%positive.
-Definition ___builtin_write16_reversed : ident := 34%positive.
-Definition ___builtin_write32_reversed : ident := 35%positive.
-Definition ___compcert_i64_dtos : ident := 46%positive.
-Definition ___compcert_i64_dtou : ident := 47%positive.
-Definition ___compcert_i64_sar : ident := 58%positive.
-Definition ___compcert_i64_sdiv : ident := 52%positive.
-Definition ___compcert_i64_shl : ident := 56%positive.
-Definition ___compcert_i64_shr : ident := 57%positive.
-Definition ___compcert_i64_smod : ident := 54%positive.
-Definition ___compcert_i64_smulh : ident := 59%positive.
-Definition ___compcert_i64_stod : ident := 48%positive.
-Definition ___compcert_i64_stof : ident := 50%positive.
-Definition ___compcert_i64_udiv : ident := 53%positive.
-Definition ___compcert_i64_umod : ident := 55%positive.
-Definition ___compcert_i64_umulh : ident := 60%positive.
-Definition ___compcert_i64_utod : ident := 49%positive.
-Definition ___compcert_i64_utof : ident := 51%positive.
-Definition ___compcert_va_composite : ident := 45%positive.
-Definition ___compcert_va_float64 : ident := 44%positive.
-Definition ___compcert_va_int32 : ident := 42%positive.
-Definition ___compcert_va_int64 : ident := 43%positive.
-Definition _a : ident := 37%positive.
-Definition _b : ident := 38%positive.
-Definition _do_and : ident := 40%positive.
-Definition _do_or : ident := 39%positive.
-Definition _main : ident := 41%positive.
-Definition _t'1 : ident := 61%positive.
+Definition ___builtin_ais_annot : ident := $"__builtin_ais_annot".
+Definition ___builtin_annot : ident := $"__builtin_annot".
+Definition ___builtin_annot_intval : ident := $"__builtin_annot_intval".
+Definition ___builtin_bswap : ident := $"__builtin_bswap".
+Definition ___builtin_bswap16 : ident := $"__builtin_bswap16".
+Definition ___builtin_bswap32 : ident := $"__builtin_bswap32".
+Definition ___builtin_bswap64 : ident := $"__builtin_bswap64".
+Definition ___builtin_clz : ident := $"__builtin_clz".
+Definition ___builtin_clzl : ident := $"__builtin_clzl".
+Definition ___builtin_clzll : ident := $"__builtin_clzll".
+Definition ___builtin_ctz : ident := $"__builtin_ctz".
+Definition ___builtin_ctzl : ident := $"__builtin_ctzl".
+Definition ___builtin_ctzll : ident := $"__builtin_ctzll".
+Definition ___builtin_debug : ident := $"__builtin_debug".
+Definition ___builtin_expect : ident := $"__builtin_expect".
+Definition ___builtin_fabs : ident := $"__builtin_fabs".
+Definition ___builtin_fabsf : ident := $"__builtin_fabsf".
+Definition ___builtin_fmadd : ident := $"__builtin_fmadd".
+Definition ___builtin_fmax : ident := $"__builtin_fmax".
+Definition ___builtin_fmin : ident := $"__builtin_fmin".
+Definition ___builtin_fmsub : ident := $"__builtin_fmsub".
+Definition ___builtin_fnmadd : ident := $"__builtin_fnmadd".
+Definition ___builtin_fnmsub : ident := $"__builtin_fnmsub".
+Definition ___builtin_fsqrt : ident := $"__builtin_fsqrt".
+Definition ___builtin_membar : ident := $"__builtin_membar".
+Definition ___builtin_memcpy_aligned : ident := $"__builtin_memcpy_aligned".
+Definition ___builtin_read16_reversed : ident := $"__builtin_read16_reversed".
+Definition ___builtin_read32_reversed : ident := $"__builtin_read32_reversed".
+Definition ___builtin_sel : ident := $"__builtin_sel".
+Definition ___builtin_sqrt : ident := $"__builtin_sqrt".
+Definition ___builtin_unreachable : ident := $"__builtin_unreachable".
+Definition ___builtin_va_arg : ident := $"__builtin_va_arg".
+Definition ___builtin_va_copy : ident := $"__builtin_va_copy".
+Definition ___builtin_va_end : ident := $"__builtin_va_end".
+Definition ___builtin_va_start : ident := $"__builtin_va_start".
+Definition ___builtin_write16_reversed : ident := $"__builtin_write16_reversed".
+Definition ___builtin_write32_reversed : ident := $"__builtin_write32_reversed".
+Definition ___compcert_i64_dtos : ident := $"__compcert_i64_dtos".
+Definition ___compcert_i64_dtou : ident := $"__compcert_i64_dtou".
+Definition ___compcert_i64_sar : ident := $"__compcert_i64_sar".
+Definition ___compcert_i64_sdiv : ident := $"__compcert_i64_sdiv".
+Definition ___compcert_i64_shl : ident := $"__compcert_i64_shl".
+Definition ___compcert_i64_shr : ident := $"__compcert_i64_shr".
+Definition ___compcert_i64_smod : ident := $"__compcert_i64_smod".
+Definition ___compcert_i64_smulh : ident := $"__compcert_i64_smulh".
+Definition ___compcert_i64_stod : ident := $"__compcert_i64_stod".
+Definition ___compcert_i64_stof : ident := $"__compcert_i64_stof".
+Definition ___compcert_i64_udiv : ident := $"__compcert_i64_udiv".
+Definition ___compcert_i64_umod : ident := $"__compcert_i64_umod".
+Definition ___compcert_i64_umulh : ident := $"__compcert_i64_umulh".
+Definition ___compcert_i64_utod : ident := $"__compcert_i64_utod".
+Definition ___compcert_i64_utof : ident := $"__compcert_i64_utof".
+Definition ___compcert_va_composite : ident := $"__compcert_va_composite".
+Definition ___compcert_va_float64 : ident := $"__compcert_va_float64".
+Definition ___compcert_va_int32 : ident := $"__compcert_va_int32".
+Definition ___compcert_va_int64 : ident := $"__compcert_va_int64".
+Definition ___stringlit_1 : ident := $"__stringlit_1".
+Definition ___stringlit_2 : ident := $"__stringlit_2".
+Definition ___stringlit_3 : ident := $"__stringlit_3".
+Definition ___stringlit_4 : ident := $"__stringlit_4".
+Definition __l : ident := $"_l".
+Definition _a : ident := $"a".
+Definition _acquire : ident := $"acquire".
+Definition _append : ident := $"append".
+Definition _args : ident := $"args".
+Definition _atom_int : ident := $"atom_int".
+Definition _b : ident := $"b".
+Definition _buf : ident := $"buf".
+Definition _c : ident := $"c".
+Definition _compute2 : ident := $"compute2".
+Definition _counter : ident := $"counter".
+Definition _ctr : ident := $"ctr".
+Definition _d : ident := $"d".
+Definition _delete : ident := $"delete".
+Definition _dest_ctr : ident := $"dest_ctr".
+Definition _do_and : ident := $"do_and".
+Definition _do_or : ident := $"do_or".
+Definition _e : ident := $"e".
+Definition _exit : ident := $"exit".
+Definition _f : ident := $"f".
+Definition _foo : ident := $"foo".
+Definition _four : ident := $"four".
+Definition _free : ident := $"free".
+Definition _freeN : ident := $"freeN".
+Definition _freelock : ident := $"freelock".
+Definition _g : ident := $"g".
+Definition _getchar : ident := $"getchar".
+Definition _getchar_blocking : ident := $"getchar_blocking".
+Definition _getchars : ident := $"getchars".
+Definition _h : ident := $"h".
+Definition _head : ident := $"head".
+Definition _hi : ident := $"hi".
+Definition _i : ident := $"i".
+Definition _i__1 : ident := $"i__1".
+Definition _incr : ident := $"incr".
+Definition _init_ctr : ident := $"init_ctr".
+Definition _insert : ident := $"insert".
+Definition _j : ident := $"j".
+Definition _k : ident := $"k".
+Definition _key : ident := $"key".
+Definition _l : ident := $"l".
+Definition _left : ident := $"left".
+Definition _list : ident := $"list".
+Definition _lo : ident := $"lo".
+Definition _lock : ident := $"lock".
+Definition _lookup : ident := $"lookup".
+Definition _main : ident := $"main".
+Definition _makelock : ident := $"makelock".
+Definition _malloc : ident := $"malloc".
+Definition _mallocN : ident := $"mallocN".
+Definition _mid : ident := $"mid".
+Definition _n : ident := $"n".
+Definition _p : ident := $"p".
+Definition _pa : ident := $"pa".
+Definition _pb : ident := $"pb".
+Definition _print_int : ident := $"print_int".
+Definition _print_intr : ident := $"print_intr".
+Definition _pushdown_left : ident := $"pushdown_left".
+Definition _putchar : ident := $"putchar".
+Definition _putchar_blocking : ident := $"putchar_blocking".
+Definition _putchars : ident := $"putchars".
+Definition _q : ident := $"q".
+Definition _r : ident := $"r".
+Definition _read : ident := $"read".
+Definition _release : ident := $"release".
+Definition _right : ident := $"right".
+Definition _s : ident := $"s".
+Definition _search : ident := $"search".
+Definition _spawn : ident := $"spawn".
+Definition _sub1 : ident := $"sub1".
+Definition _sub2 : ident := $"sub2".
+Definition _sub3 : ident := $"sub3".
+Definition _t : ident := $"t".
+Definition _tail : ident := $"tail".
+Definition _tgt : ident := $"tgt".
+Definition _thread_func : ident := $"thread_func".
+Definition _thread_lock : ident := $"thread_lock".
+Definition _tree : ident := $"tree".
+Definition _tree_free : ident := $"tree_free".
+Definition _treebox_free : ident := $"treebox_free".
+Definition _treebox_new : ident := $"treebox_new".
+Definition _turn_left : ident := $"turn_left".
+Definition _u : ident := $"u".
+Definition _v : ident := $"v".
+Definition _val : ident := $"val".
+Definition _value : ident := $"value".
+Definition _x : ident := $"x".
+Definition _x1 : ident := $"x1".
+Definition _x2 : ident := $"x2".
+Definition _y : ident := $"y".
+Definition _y1 : ident := $"y1".
+Definition _y2 : ident := $"y2".
+Definition _z : ident := $"z".
+Definition _t'1 : ident := 128%positive.
 
 Definition f_do_or := {|
   fn_return := tbool;
@@ -127,264 +220,259 @@ nil.
 Definition global_definitions : list (ident * globdef fundef type) :=
 ((___compcert_va_int32,
    Gfun(External (EF_runtime "__compcert_va_int32"
-                   (mksignature (AST.Tlong :: nil) AST.Tint cc_default))
-     (Tcons (tptr tvoid) Tnil) tuint cc_default)) ::
+                   (mksignature (AST.Xptr :: nil) AST.Xint cc_default))
+     ((tptr tvoid) :: nil) tuint cc_default)) ::
  (___compcert_va_int64,
    Gfun(External (EF_runtime "__compcert_va_int64"
-                   (mksignature (AST.Tlong :: nil) AST.Tlong cc_default))
-     (Tcons (tptr tvoid) Tnil) tulong cc_default)) ::
+                   (mksignature (AST.Xptr :: nil) AST.Xlong cc_default))
+     ((tptr tvoid) :: nil) tulong cc_default)) ::
  (___compcert_va_float64,
    Gfun(External (EF_runtime "__compcert_va_float64"
-                   (mksignature (AST.Tlong :: nil) AST.Tfloat cc_default))
-     (Tcons (tptr tvoid) Tnil) tdouble cc_default)) ::
+                   (mksignature (AST.Xptr :: nil) AST.Xfloat cc_default))
+     ((tptr tvoid) :: nil) tdouble cc_default)) ::
  (___compcert_va_composite,
    Gfun(External (EF_runtime "__compcert_va_composite"
-                   (mksignature (AST.Tlong :: AST.Tlong :: nil) AST.Tlong
-                     cc_default)) (Tcons (tptr tvoid) (Tcons tulong Tnil))
+                   (mksignature (AST.Xptr :: AST.Xlong :: nil) AST.Xptr
+                     cc_default)) ((tptr tvoid) :: tulong :: nil)
      (tptr tvoid) cc_default)) ::
  (___compcert_i64_dtos,
    Gfun(External (EF_runtime "__compcert_i64_dtos"
-                   (mksignature (AST.Tfloat :: nil) AST.Tlong cc_default))
-     (Tcons tdouble Tnil) tlong cc_default)) ::
+                   (mksignature (AST.Xfloat :: nil) AST.Xlong cc_default))
+     (tdouble :: nil) tlong cc_default)) ::
  (___compcert_i64_dtou,
    Gfun(External (EF_runtime "__compcert_i64_dtou"
-                   (mksignature (AST.Tfloat :: nil) AST.Tlong cc_default))
-     (Tcons tdouble Tnil) tulong cc_default)) ::
+                   (mksignature (AST.Xfloat :: nil) AST.Xlong cc_default))
+     (tdouble :: nil) tulong cc_default)) ::
  (___compcert_i64_stod,
    Gfun(External (EF_runtime "__compcert_i64_stod"
-                   (mksignature (AST.Tlong :: nil) AST.Tfloat cc_default))
-     (Tcons tlong Tnil) tdouble cc_default)) ::
+                   (mksignature (AST.Xlong :: nil) AST.Xfloat cc_default))
+     (tlong :: nil) tdouble cc_default)) ::
  (___compcert_i64_utod,
    Gfun(External (EF_runtime "__compcert_i64_utod"
-                   (mksignature (AST.Tlong :: nil) AST.Tfloat cc_default))
-     (Tcons tulong Tnil) tdouble cc_default)) ::
+                   (mksignature (AST.Xlong :: nil) AST.Xfloat cc_default))
+     (tulong :: nil) tdouble cc_default)) ::
  (___compcert_i64_stof,
    Gfun(External (EF_runtime "__compcert_i64_stof"
-                   (mksignature (AST.Tlong :: nil) AST.Tsingle cc_default))
-     (Tcons tlong Tnil) tfloat cc_default)) ::
+                   (mksignature (AST.Xlong :: nil) AST.Xsingle cc_default))
+     (tlong :: nil) tfloat cc_default)) ::
  (___compcert_i64_utof,
    Gfun(External (EF_runtime "__compcert_i64_utof"
-                   (mksignature (AST.Tlong :: nil) AST.Tsingle cc_default))
-     (Tcons tulong Tnil) tfloat cc_default)) ::
+                   (mksignature (AST.Xlong :: nil) AST.Xsingle cc_default))
+     (tulong :: nil) tfloat cc_default)) ::
  (___compcert_i64_sdiv,
    Gfun(External (EF_runtime "__compcert_i64_sdiv"
-                   (mksignature (AST.Tlong :: AST.Tlong :: nil) AST.Tlong
-                     cc_default)) (Tcons tlong (Tcons tlong Tnil)) tlong
-     cc_default)) ::
+                   (mksignature (AST.Xlong :: AST.Xlong :: nil) AST.Xlong
+                     cc_default)) (tlong :: tlong :: nil) tlong cc_default)) ::
  (___compcert_i64_udiv,
    Gfun(External (EF_runtime "__compcert_i64_udiv"
-                   (mksignature (AST.Tlong :: AST.Tlong :: nil) AST.Tlong
-                     cc_default)) (Tcons tulong (Tcons tulong Tnil)) tulong
+                   (mksignature (AST.Xlong :: AST.Xlong :: nil) AST.Xlong
+                     cc_default)) (tulong :: tulong :: nil) tulong
      cc_default)) ::
  (___compcert_i64_smod,
    Gfun(External (EF_runtime "__compcert_i64_smod"
-                   (mksignature (AST.Tlong :: AST.Tlong :: nil) AST.Tlong
-                     cc_default)) (Tcons tlong (Tcons tlong Tnil)) tlong
-     cc_default)) ::
+                   (mksignature (AST.Xlong :: AST.Xlong :: nil) AST.Xlong
+                     cc_default)) (tlong :: tlong :: nil) tlong cc_default)) ::
  (___compcert_i64_umod,
    Gfun(External (EF_runtime "__compcert_i64_umod"
-                   (mksignature (AST.Tlong :: AST.Tlong :: nil) AST.Tlong
-                     cc_default)) (Tcons tulong (Tcons tulong Tnil)) tulong
+                   (mksignature (AST.Xlong :: AST.Xlong :: nil) AST.Xlong
+                     cc_default)) (tulong :: tulong :: nil) tulong
      cc_default)) ::
  (___compcert_i64_shl,
    Gfun(External (EF_runtime "__compcert_i64_shl"
-                   (mksignature (AST.Tlong :: AST.Tint :: nil) AST.Tlong
-                     cc_default)) (Tcons tlong (Tcons tint Tnil)) tlong
-     cc_default)) ::
+                   (mksignature (AST.Xlong :: AST.Xint :: nil) AST.Xlong
+                     cc_default)) (tlong :: tint :: nil) tlong cc_default)) ::
  (___compcert_i64_shr,
    Gfun(External (EF_runtime "__compcert_i64_shr"
-                   (mksignature (AST.Tlong :: AST.Tint :: nil) AST.Tlong
-                     cc_default)) (Tcons tulong (Tcons tint Tnil)) tulong
-     cc_default)) ::
+                   (mksignature (AST.Xlong :: AST.Xint :: nil) AST.Xlong
+                     cc_default)) (tulong :: tint :: nil) tulong cc_default)) ::
  (___compcert_i64_sar,
    Gfun(External (EF_runtime "__compcert_i64_sar"
-                   (mksignature (AST.Tlong :: AST.Tint :: nil) AST.Tlong
-                     cc_default)) (Tcons tlong (Tcons tint Tnil)) tlong
-     cc_default)) ::
+                   (mksignature (AST.Xlong :: AST.Xint :: nil) AST.Xlong
+                     cc_default)) (tlong :: tint :: nil) tlong cc_default)) ::
  (___compcert_i64_smulh,
    Gfun(External (EF_runtime "__compcert_i64_smulh"
-                   (mksignature (AST.Tlong :: AST.Tlong :: nil) AST.Tlong
-                     cc_default)) (Tcons tlong (Tcons tlong Tnil)) tlong
-     cc_default)) ::
+                   (mksignature (AST.Xlong :: AST.Xlong :: nil) AST.Xlong
+                     cc_default)) (tlong :: tlong :: nil) tlong cc_default)) ::
  (___compcert_i64_umulh,
    Gfun(External (EF_runtime "__compcert_i64_umulh"
-                   (mksignature (AST.Tlong :: AST.Tlong :: nil) AST.Tlong
-                     cc_default)) (Tcons tulong (Tcons tulong Tnil)) tulong
+                   (mksignature (AST.Xlong :: AST.Xlong :: nil) AST.Xlong
+                     cc_default)) (tulong :: tulong :: nil) tulong
      cc_default)) ::
+ (___builtin_ais_annot,
+   Gfun(External (EF_builtin "__builtin_ais_annot"
+                   (mksignature (AST.Xptr :: nil) AST.Xvoid
+                     {|cc_vararg:=(Some 1); cc_unproto:=false; cc_structret:=false|}))
+     ((tptr tschar) :: nil) tvoid
+     {|cc_vararg:=(Some 1); cc_unproto:=false; cc_structret:=false|})) ::
  (___builtin_bswap64,
    Gfun(External (EF_builtin "__builtin_bswap64"
-                   (mksignature (AST.Tlong :: nil) AST.Tlong cc_default))
-     (Tcons tulong Tnil) tulong cc_default)) ::
+                   (mksignature (AST.Xlong :: nil) AST.Xlong cc_default))
+     (tulong :: nil) tulong cc_default)) ::
  (___builtin_bswap,
    Gfun(External (EF_builtin "__builtin_bswap"
-                   (mksignature (AST.Tint :: nil) AST.Tint cc_default))
-     (Tcons tuint Tnil) tuint cc_default)) ::
+                   (mksignature (AST.Xint :: nil) AST.Xint cc_default))
+     (tuint :: nil) tuint cc_default)) ::
  (___builtin_bswap32,
    Gfun(External (EF_builtin "__builtin_bswap32"
-                   (mksignature (AST.Tint :: nil) AST.Tint cc_default))
-     (Tcons tuint Tnil) tuint cc_default)) ::
+                   (mksignature (AST.Xint :: nil) AST.Xint cc_default))
+     (tuint :: nil) tuint cc_default)) ::
  (___builtin_bswap16,
    Gfun(External (EF_builtin "__builtin_bswap16"
-                   (mksignature (AST.Tint :: nil) AST.Tint16unsigned
-                     cc_default)) (Tcons tushort Tnil) tushort cc_default)) ::
+                   (mksignature (AST.Xint16unsigned :: nil)
+                     AST.Xint16unsigned cc_default)) (tushort :: nil) tushort
+     cc_default)) ::
  (___builtin_clz,
    Gfun(External (EF_builtin "__builtin_clz"
-                   (mksignature (AST.Tint :: nil) AST.Tint cc_default))
-     (Tcons tuint Tnil) tint cc_default)) ::
+                   (mksignature (AST.Xint :: nil) AST.Xint cc_default))
+     (tuint :: nil) tint cc_default)) ::
  (___builtin_clzl,
    Gfun(External (EF_builtin "__builtin_clzl"
-                   (mksignature (AST.Tlong :: nil) AST.Tint cc_default))
-     (Tcons tulong Tnil) tint cc_default)) ::
+                   (mksignature (AST.Xlong :: nil) AST.Xint cc_default))
+     (tulong :: nil) tint cc_default)) ::
  (___builtin_clzll,
    Gfun(External (EF_builtin "__builtin_clzll"
-                   (mksignature (AST.Tlong :: nil) AST.Tint cc_default))
-     (Tcons tulong Tnil) tint cc_default)) ::
+                   (mksignature (AST.Xlong :: nil) AST.Xint cc_default))
+     (tulong :: nil) tint cc_default)) ::
  (___builtin_ctz,
    Gfun(External (EF_builtin "__builtin_ctz"
-                   (mksignature (AST.Tint :: nil) AST.Tint cc_default))
-     (Tcons tuint Tnil) tint cc_default)) ::
+                   (mksignature (AST.Xint :: nil) AST.Xint cc_default))
+     (tuint :: nil) tint cc_default)) ::
  (___builtin_ctzl,
    Gfun(External (EF_builtin "__builtin_ctzl"
-                   (mksignature (AST.Tlong :: nil) AST.Tint cc_default))
-     (Tcons tulong Tnil) tint cc_default)) ::
+                   (mksignature (AST.Xlong :: nil) AST.Xint cc_default))
+     (tulong :: nil) tint cc_default)) ::
  (___builtin_ctzll,
    Gfun(External (EF_builtin "__builtin_ctzll"
-                   (mksignature (AST.Tlong :: nil) AST.Tint cc_default))
-     (Tcons tulong Tnil) tint cc_default)) ::
+                   (mksignature (AST.Xlong :: nil) AST.Xint cc_default))
+     (tulong :: nil) tint cc_default)) ::
  (___builtin_fabs,
    Gfun(External (EF_builtin "__builtin_fabs"
-                   (mksignature (AST.Tfloat :: nil) AST.Tfloat cc_default))
-     (Tcons tdouble Tnil) tdouble cc_default)) ::
+                   (mksignature (AST.Xfloat :: nil) AST.Xfloat cc_default))
+     (tdouble :: nil) tdouble cc_default)) ::
  (___builtin_fabsf,
    Gfun(External (EF_builtin "__builtin_fabsf"
-                   (mksignature (AST.Tsingle :: nil) AST.Tsingle cc_default))
-     (Tcons tfloat Tnil) tfloat cc_default)) ::
+                   (mksignature (AST.Xsingle :: nil) AST.Xsingle cc_default))
+     (tfloat :: nil) tfloat cc_default)) ::
  (___builtin_fsqrt,
    Gfun(External (EF_builtin "__builtin_fsqrt"
-                   (mksignature (AST.Tfloat :: nil) AST.Tfloat cc_default))
-     (Tcons tdouble Tnil) tdouble cc_default)) ::
+                   (mksignature (AST.Xfloat :: nil) AST.Xfloat cc_default))
+     (tdouble :: nil) tdouble cc_default)) ::
  (___builtin_sqrt,
    Gfun(External (EF_builtin "__builtin_sqrt"
-                   (mksignature (AST.Tfloat :: nil) AST.Tfloat cc_default))
-     (Tcons tdouble Tnil) tdouble cc_default)) ::
+                   (mksignature (AST.Xfloat :: nil) AST.Xfloat cc_default))
+     (tdouble :: nil) tdouble cc_default)) ::
  (___builtin_memcpy_aligned,
    Gfun(External (EF_builtin "__builtin_memcpy_aligned"
                    (mksignature
-                     (AST.Tlong :: AST.Tlong :: AST.Tlong :: AST.Tlong ::
-                      nil) AST.Tvoid cc_default))
-     (Tcons (tptr tvoid)
-       (Tcons (tptr tvoid) (Tcons tulong (Tcons tulong Tnil)))) tvoid
+                     (AST.Xptr :: AST.Xptr :: AST.Xlong :: AST.Xlong :: nil)
+                     AST.Xvoid cc_default))
+     ((tptr tvoid) :: (tptr tvoid) :: tulong :: tulong :: nil) tvoid
      cc_default)) ::
  (___builtin_sel,
    Gfun(External (EF_builtin "__builtin_sel"
-                   (mksignature (AST.Tint :: nil) AST.Tvoid
+                   (mksignature (AST.Xbool :: nil) AST.Xvoid
                      {|cc_vararg:=(Some 1); cc_unproto:=false; cc_structret:=false|}))
-     (Tcons tbool Tnil) tvoid
+     (tbool :: nil) tvoid
      {|cc_vararg:=(Some 1); cc_unproto:=false; cc_structret:=false|})) ::
  (___builtin_annot,
    Gfun(External (EF_builtin "__builtin_annot"
-                   (mksignature (AST.Tlong :: nil) AST.Tvoid
+                   (mksignature (AST.Xptr :: nil) AST.Xvoid
                      {|cc_vararg:=(Some 1); cc_unproto:=false; cc_structret:=false|}))
-     (Tcons (tptr tschar) Tnil) tvoid
+     ((tptr tschar) :: nil) tvoid
      {|cc_vararg:=(Some 1); cc_unproto:=false; cc_structret:=false|})) ::
  (___builtin_annot_intval,
    Gfun(External (EF_builtin "__builtin_annot_intval"
-                   (mksignature (AST.Tlong :: AST.Tint :: nil) AST.Tint
-                     cc_default)) (Tcons (tptr tschar) (Tcons tint Tnil))
-     tint cc_default)) ::
+                   (mksignature (AST.Xptr :: AST.Xint :: nil) AST.Xint
+                     cc_default)) ((tptr tschar) :: tint :: nil) tint
+     cc_default)) ::
  (___builtin_membar,
    Gfun(External (EF_builtin "__builtin_membar"
-                   (mksignature nil AST.Tvoid cc_default)) Tnil tvoid
+                   (mksignature nil AST.Xvoid cc_default)) nil tvoid
      cc_default)) ::
  (___builtin_va_start,
    Gfun(External (EF_builtin "__builtin_va_start"
-                   (mksignature (AST.Tlong :: nil) AST.Tvoid cc_default))
-     (Tcons (tptr tvoid) Tnil) tvoid cc_default)) ::
+                   (mksignature (AST.Xptr :: nil) AST.Xvoid cc_default))
+     ((tptr tvoid) :: nil) tvoid cc_default)) ::
  (___builtin_va_arg,
    Gfun(External (EF_builtin "__builtin_va_arg"
-                   (mksignature (AST.Tlong :: AST.Tint :: nil) AST.Tvoid
-                     cc_default)) (Tcons (tptr tvoid) (Tcons tuint Tnil))
-     tvoid cc_default)) ::
+                   (mksignature (AST.Xptr :: AST.Xint :: nil) AST.Xvoid
+                     cc_default)) ((tptr tvoid) :: tuint :: nil) tvoid
+     cc_default)) ::
  (___builtin_va_copy,
    Gfun(External (EF_builtin "__builtin_va_copy"
-                   (mksignature (AST.Tlong :: AST.Tlong :: nil) AST.Tvoid
-                     cc_default))
-     (Tcons (tptr tvoid) (Tcons (tptr tvoid) Tnil)) tvoid cc_default)) ::
+                   (mksignature (AST.Xptr :: AST.Xptr :: nil) AST.Xvoid
+                     cc_default)) ((tptr tvoid) :: (tptr tvoid) :: nil) tvoid
+     cc_default)) ::
  (___builtin_va_end,
    Gfun(External (EF_builtin "__builtin_va_end"
-                   (mksignature (AST.Tlong :: nil) AST.Tvoid cc_default))
-     (Tcons (tptr tvoid) Tnil) tvoid cc_default)) ::
+                   (mksignature (AST.Xptr :: nil) AST.Xvoid cc_default))
+     ((tptr tvoid) :: nil) tvoid cc_default)) ::
  (___builtin_unreachable,
    Gfun(External (EF_builtin "__builtin_unreachable"
-                   (mksignature nil AST.Tvoid cc_default)) Tnil tvoid
+                   (mksignature nil AST.Xvoid cc_default)) nil tvoid
      cc_default)) ::
  (___builtin_expect,
    Gfun(External (EF_builtin "__builtin_expect"
-                   (mksignature (AST.Tlong :: AST.Tlong :: nil) AST.Tlong
-                     cc_default)) (Tcons tlong (Tcons tlong Tnil)) tlong
-     cc_default)) ::
+                   (mksignature (AST.Xlong :: AST.Xlong :: nil) AST.Xlong
+                     cc_default)) (tlong :: tlong :: nil) tlong cc_default)) ::
  (___builtin_fmax,
    Gfun(External (EF_builtin "__builtin_fmax"
-                   (mksignature (AST.Tfloat :: AST.Tfloat :: nil) AST.Tfloat
-                     cc_default)) (Tcons tdouble (Tcons tdouble Tnil))
-     tdouble cc_default)) ::
+                   (mksignature (AST.Xfloat :: AST.Xfloat :: nil) AST.Xfloat
+                     cc_default)) (tdouble :: tdouble :: nil) tdouble
+     cc_default)) ::
  (___builtin_fmin,
    Gfun(External (EF_builtin "__builtin_fmin"
-                   (mksignature (AST.Tfloat :: AST.Tfloat :: nil) AST.Tfloat
-                     cc_default)) (Tcons tdouble (Tcons tdouble Tnil))
-     tdouble cc_default)) ::
+                   (mksignature (AST.Xfloat :: AST.Xfloat :: nil) AST.Xfloat
+                     cc_default)) (tdouble :: tdouble :: nil) tdouble
+     cc_default)) ::
  (___builtin_fmadd,
    Gfun(External (EF_builtin "__builtin_fmadd"
                    (mksignature
-                     (AST.Tfloat :: AST.Tfloat :: AST.Tfloat :: nil)
-                     AST.Tfloat cc_default))
-     (Tcons tdouble (Tcons tdouble (Tcons tdouble Tnil))) tdouble
-     cc_default)) ::
+                     (AST.Xfloat :: AST.Xfloat :: AST.Xfloat :: nil)
+                     AST.Xfloat cc_default))
+     (tdouble :: tdouble :: tdouble :: nil) tdouble cc_default)) ::
  (___builtin_fmsub,
    Gfun(External (EF_builtin "__builtin_fmsub"
                    (mksignature
-                     (AST.Tfloat :: AST.Tfloat :: AST.Tfloat :: nil)
-                     AST.Tfloat cc_default))
-     (Tcons tdouble (Tcons tdouble (Tcons tdouble Tnil))) tdouble
-     cc_default)) ::
+                     (AST.Xfloat :: AST.Xfloat :: AST.Xfloat :: nil)
+                     AST.Xfloat cc_default))
+     (tdouble :: tdouble :: tdouble :: nil) tdouble cc_default)) ::
  (___builtin_fnmadd,
    Gfun(External (EF_builtin "__builtin_fnmadd"
                    (mksignature
-                     (AST.Tfloat :: AST.Tfloat :: AST.Tfloat :: nil)
-                     AST.Tfloat cc_default))
-     (Tcons tdouble (Tcons tdouble (Tcons tdouble Tnil))) tdouble
-     cc_default)) ::
+                     (AST.Xfloat :: AST.Xfloat :: AST.Xfloat :: nil)
+                     AST.Xfloat cc_default))
+     (tdouble :: tdouble :: tdouble :: nil) tdouble cc_default)) ::
  (___builtin_fnmsub,
    Gfun(External (EF_builtin "__builtin_fnmsub"
                    (mksignature
-                     (AST.Tfloat :: AST.Tfloat :: AST.Tfloat :: nil)
-                     AST.Tfloat cc_default))
-     (Tcons tdouble (Tcons tdouble (Tcons tdouble Tnil))) tdouble
-     cc_default)) ::
+                     (AST.Xfloat :: AST.Xfloat :: AST.Xfloat :: nil)
+                     AST.Xfloat cc_default))
+     (tdouble :: tdouble :: tdouble :: nil) tdouble cc_default)) ::
  (___builtin_read16_reversed,
    Gfun(External (EF_builtin "__builtin_read16_reversed"
-                   (mksignature (AST.Tlong :: nil) AST.Tint16unsigned
-                     cc_default)) (Tcons (tptr tushort) Tnil) tushort
+                   (mksignature (AST.Xptr :: nil) AST.Xint16unsigned
+                     cc_default)) ((tptr tushort) :: nil) tushort
      cc_default)) ::
  (___builtin_read32_reversed,
    Gfun(External (EF_builtin "__builtin_read32_reversed"
-                   (mksignature (AST.Tlong :: nil) AST.Tint cc_default))
-     (Tcons (tptr tuint) Tnil) tuint cc_default)) ::
+                   (mksignature (AST.Xptr :: nil) AST.Xint cc_default))
+     ((tptr tuint) :: nil) tuint cc_default)) ::
  (___builtin_write16_reversed,
    Gfun(External (EF_builtin "__builtin_write16_reversed"
-                   (mksignature (AST.Tlong :: AST.Tint :: nil) AST.Tvoid
-                     cc_default)) (Tcons (tptr tushort) (Tcons tushort Tnil))
-     tvoid cc_default)) ::
+                   (mksignature (AST.Xptr :: AST.Xint16unsigned :: nil)
+                     AST.Xvoid cc_default))
+     ((tptr tushort) :: tushort :: nil) tvoid cc_default)) ::
  (___builtin_write32_reversed,
    Gfun(External (EF_builtin "__builtin_write32_reversed"
-                   (mksignature (AST.Tlong :: AST.Tint :: nil) AST.Tvoid
-                     cc_default)) (Tcons (tptr tuint) (Tcons tuint Tnil))
-     tvoid cc_default)) ::
+                   (mksignature (AST.Xptr :: AST.Xint :: nil) AST.Xvoid
+                     cc_default)) ((tptr tuint) :: tuint :: nil) tvoid
+     cc_default)) ::
  (___builtin_debug,
    Gfun(External (EF_external "__builtin_debug"
-                   (mksignature (AST.Tint :: nil) AST.Tvoid
+                   (mksignature (AST.Xint :: nil) AST.Xvoid
                      {|cc_vararg:=(Some 1); cc_unproto:=false; cc_structret:=false|}))
-     (Tcons tint Tnil) tvoid
+     (tint :: nil) tvoid
      {|cc_vararg:=(Some 1); cc_unproto:=false; cc_structret:=false|})) ::
  (_do_or, Gfun(Internal f_do_or)) :: (_do_and, Gfun(Internal f_do_and)) ::
  (_main, Gfun(Internal f_main)) :: nil).
@@ -403,13 +491,14 @@ Definition public_idents : list ident :=
  ___builtin_ctzll :: ___builtin_ctzl :: ___builtin_ctz :: ___builtin_clzll ::
  ___builtin_clzl :: ___builtin_clz :: ___builtin_bswap16 ::
  ___builtin_bswap32 :: ___builtin_bswap :: ___builtin_bswap64 ::
- ___compcert_i64_umulh :: ___compcert_i64_smulh :: ___compcert_i64_sar ::
- ___compcert_i64_shr :: ___compcert_i64_shl :: ___compcert_i64_umod ::
- ___compcert_i64_smod :: ___compcert_i64_udiv :: ___compcert_i64_sdiv ::
- ___compcert_i64_utof :: ___compcert_i64_stof :: ___compcert_i64_utod ::
- ___compcert_i64_stod :: ___compcert_i64_dtou :: ___compcert_i64_dtos ::
- ___compcert_va_composite :: ___compcert_va_float64 ::
- ___compcert_va_int64 :: ___compcert_va_int32 :: nil).
+ ___builtin_ais_annot :: ___compcert_i64_umulh :: ___compcert_i64_smulh ::
+ ___compcert_i64_sar :: ___compcert_i64_shr :: ___compcert_i64_shl ::
+ ___compcert_i64_umod :: ___compcert_i64_smod :: ___compcert_i64_udiv ::
+ ___compcert_i64_sdiv :: ___compcert_i64_utof :: ___compcert_i64_stof ::
+ ___compcert_i64_utod :: ___compcert_i64_stod :: ___compcert_i64_dtou ::
+ ___compcert_i64_dtos :: ___compcert_va_composite ::
+ ___compcert_va_float64 :: ___compcert_va_int64 :: ___compcert_va_int32 ::
+ nil).
 
 Definition prog : Clight.program := 
   mkprogram composites global_definitions public_idents _main Logic.I.
