progs64/printf.v
@@ -6,7 +6,7 @@ Local Open Scope string_scope.
 Local Open Scope clight_scope.
 
 Module Info.
-  Definition version := "3.9".
+  Definition version := "3.15".
   Definition build_number := "".
   Definition build_tag := "".
   Definition build_branch := "".
@@ -19,185 +19,238 @@ Module Info.
   Definition normalized := true.
 End Info.
 
-Definition __139 : ident := 6%positive.
-Definition __140 : ident := 3%positive.
-Definition __213 : ident := 93%positive.
-Definition __214 : ident := 88%positive.
-Definition __215 : ident := 91%positive.
-Definition __Bigint : ident := 8%positive.
-Definition ___builtin_annot : ident := 132%positive.
-Definition ___builtin_annot_intval : ident := 133%positive.
-Definition ___builtin_bswap : ident := 117%positive.
-Definition ___builtin_bswap16 : ident := 119%positive.
-Definition ___builtin_bswap32 : ident := 118%positive.
-Definition ___builtin_bswap64 : ident := 116%positive.
-Definition ___builtin_clz : ident := 120%positive.
-Definition ___builtin_clzl : ident := 121%positive.
-Definition ___builtin_clzll : ident := 122%positive.
-Definition ___builtin_ctz : ident := 123%positive.
-Definition ___builtin_ctzl : ident := 124%positive.
-Definition ___builtin_ctzll : ident := 125%positive.
-Definition ___builtin_debug : ident := 151%positive.
-Definition ___builtin_expect : ident := 140%positive.
-Definition ___builtin_fabs : ident := 126%positive.
-Definition ___builtin_fabsf : ident := 127%positive.
-Definition ___builtin_fmadd : ident := 143%positive.
-Definition ___builtin_fmax : ident := 141%positive.
-Definition ___builtin_fmin : ident := 142%positive.
-Definition ___builtin_fmsub : ident := 144%positive.
-Definition ___builtin_fnmadd : ident := 145%positive.
-Definition ___builtin_fnmsub : ident := 146%positive.
-Definition ___builtin_fsqrt : ident := 128%positive.
-Definition ___builtin_membar : ident := 134%positive.
-Definition ___builtin_memcpy_aligned : ident := 130%positive.
-Definition ___builtin_read16_reversed : ident := 147%positive.
-Definition ___builtin_read32_reversed : ident := 148%positive.
-Definition ___builtin_sel : ident := 131%positive.
-Definition ___builtin_sqrt : ident := 129%positive.
-Definition ___builtin_unreachable : ident := 139%positive.
-Definition ___builtin_va_arg : ident := 136%positive.
-Definition ___builtin_va_copy : ident := 137%positive.
-Definition ___builtin_va_end : ident := 138%positive.
-Definition ___builtin_va_start : ident := 135%positive.
-Definition ___builtin_write16_reversed : ident := 149%positive.
-Definition ___builtin_write32_reversed : ident := 150%positive.
-Definition ___cleanup : ident := 104%positive.
-Definition ___compcert_i64_dtos : ident := 163%positive.
-Definition ___compcert_i64_dtou : ident := 164%positive.
-Definition ___compcert_i64_sar : ident := 175%positive.
-Definition ___compcert_i64_sdiv : ident := 169%positive.
-Definition ___compcert_i64_shl : ident := 173%positive.
-Definition ___compcert_i64_shr : ident := 174%positive.
-Definition ___compcert_i64_smod : ident := 171%positive.
-Definition ___compcert_i64_smulh : ident := 176%positive.
-Definition ___compcert_i64_stod : ident := 165%positive.
-Definition ___compcert_i64_stof : ident := 167%positive.
-Definition ___compcert_i64_udiv : ident := 170%positive.
-Definition ___compcert_i64_umod : ident := 172%positive.
-Definition ___compcert_i64_umulh : ident := 177%positive.
-Definition ___compcert_i64_utod : ident := 166%positive.
-Definition ___compcert_i64_utof : ident := 168%positive.
-Definition ___compcert_va_composite : ident := 162%positive.
-Definition ___compcert_va_float64 : ident := 161%positive.
-Definition ___compcert_va_int32 : ident := 159%positive.
-Definition ___compcert_va_int64 : ident := 160%positive.
-Definition ___count : ident := 4%positive.
-Definition ___getreent : ident := 152%positive.
-Definition ___locale_t : ident := 102%positive.
-Definition ___sFILE64 : ident := 61%positive.
-Definition ___sbuf : ident := 34%positive.
-Definition ___sdidinit : ident := 103%positive.
-Definition ___sf : ident := 115%positive.
-Definition ___sglue : ident := 114%positive.
-Definition ___stringlit_1 : ident := 155%positive.
-Definition ___stringlit_2 : ident := 156%positive.
-Definition ___stringlit_3 : ident := 157%positive.
-Definition ___tm : ident := 23%positive.
-Definition ___tm_hour : ident := 16%positive.
-Definition ___tm_isdst : ident := 22%positive.
-Definition ___tm_mday : ident := 17%positive.
-Definition ___tm_min : ident := 15%positive.
-Definition ___tm_mon : ident := 18%positive.
-Definition ___tm_sec : ident := 14%positive.
-Definition ___tm_wday : ident := 20%positive.
-Definition ___tm_yday : ident := 21%positive.
-Definition ___tm_year : ident := 19%positive.
-Definition ___value : ident := 5%positive.
-Definition ___wch : ident := 1%positive.
-Definition ___wchb : ident := 2%positive.
-Definition __add : ident := 67%positive.
-Definition __asctime_buf : ident := 71%positive.
-Definition __atexit : ident := 29%positive.
-Definition __atexit0 : ident := 112%positive.
-Definition __base : ident := 32%positive.
-Definition __bf : ident := 40%positive.
-Definition __blksize : ident := 55%positive.
-Definition __close : ident := 48%positive.
-Definition __cookie : ident := 44%positive.
-Definition __cvtbuf : ident := 110%positive.
-Definition __cvtlen : ident := 109%positive.
-Definition __data : ident := 42%positive.
-Definition __dso_handle : ident := 25%positive.
-Definition __emergency : ident := 99%positive.
-Definition __errno : ident := 94%positive.
-Definition __file : ident := 39%positive.
-Definition __flags : ident := 38%positive.
-Definition __flags2 : ident := 56%positive.
-Definition __fnargs : ident := 24%positive.
-Definition __fns : ident := 31%positive.
-Definition __fntypes : ident := 26%positive.
-Definition __freelist : ident := 108%positive.
-Definition __gamma_signgam : ident := 73%positive.
-Definition __getdate_err : ident := 81%positive.
-Definition __glue : ident := 62%positive.
-Definition __h_errno : ident := 87%positive.
-Definition __inc : ident := 98%positive.
-Definition __ind : ident := 30%positive.
-Definition __iobs : ident := 64%positive.
-Definition __is_cxa : ident := 27%positive.
-Definition __k : ident := 9%positive.
-Definition __l64a_buf : ident := 79%positive.
-Definition __lb : ident := 54%positive.
-Definition __lbfsize : ident := 41%positive.
-Definition __locale : ident := 101%positive.
-Definition __localtime_buf : ident := 72%positive.
-Definition __lock : ident := 59%positive.
-Definition __maxwds : ident := 10%positive.
-Definition __mblen_state : ident := 76%positive.
-Definition __mbrlen_state : ident := 82%positive.
-Definition __mbrtowc_state : ident := 83%positive.
-Definition __mbsrtowcs_state : ident := 84%positive.
-Definition __mbstate : ident := 60%positive.
-Definition __mbtowc_state : ident := 77%positive.
-Definition __mult : ident := 66%positive.
-Definition __nbuf : ident := 53%positive.
-Definition __new : ident := 111%positive.
-Definition __next : ident := 7%positive.
-Definition __nextf : ident := 89%positive.
-Definition __niobs : ident := 63%positive.
-Definition __nmalloc : ident := 90%positive.
-Definition __offset : ident := 57%positive.
-Definition __on_exit_args : ident := 28%positive.
-Definition __p : ident := 35%positive.
-Definition __p5s : ident := 107%positive.
-Definition __r : ident := 36%positive.
-Definition __r48 : ident := 75%positive.
-Definition __rand48 : ident := 68%positive.
-Definition __rand_next : ident := 74%positive.
-Definition __read : ident := 45%positive.
-Definition __reent : ident := 43%positive.
-Definition __result : ident := 105%positive.
-Definition __result_k : ident := 106%positive.
-Definition __seed : ident := 65%positive.
-Definition __seek : ident := 47%positive.
-Definition __seek64 : ident := 58%positive.
-Definition __sig_func : ident := 113%positive.
-Definition __sign : ident := 11%positive.
-Definition __signal_buf : ident := 80%positive.
-Definition __size : ident := 33%positive.
-Definition __stderr : ident := 97%positive.
-Definition __stdin : ident := 95%positive.
-Definition __stdout : ident := 96%positive.
-Definition __strtok_last : ident := 70%positive.
-Definition __ub : ident := 49%positive.
-Definition __ubuf : ident := 52%positive.
-Definition __unspecified_locale_info : ident := 100%positive.
-Definition __unused : ident := 92%positive.
-Definition __unused_rand : ident := 69%positive.
-Definition __up : ident := 50%positive.
-Definition __ur : ident := 51%positive.
-Definition __w : ident := 37%positive.
-Definition __wcrtomb_state : ident := 85%positive.
-Definition __wcsrtombs_state : ident := 86%positive.
-Definition __wctomb_state : ident := 78%positive.
-Definition __wds : ident := 12%positive.
-Definition __write : ident := 46%positive.
-Definition __x : ident := 13%positive.
-Definition _fprintf : ident := 153%positive.
-Definition _main : ident := 158%positive.
-Definition _printf : ident := 154%positive.
-Definition _t'1 : ident := 178%positive.
-Definition _t'2 : ident := 179%positive.
+Definition __IO_FILE : ident := $"_IO_FILE".
+Definition __IO_backup_base : ident := $"_IO_backup_base".
+Definition __IO_buf_base : ident := $"_IO_buf_base".
+Definition __IO_buf_end : ident := $"_IO_buf_end".
+Definition __IO_codecvt : ident := $"_IO_codecvt".
+Definition __IO_marker : ident := $"_IO_marker".
+Definition __IO_read_base : ident := $"_IO_read_base".
+Definition __IO_read_end : ident := $"_IO_read_end".
+Definition __IO_read_ptr : ident := $"_IO_read_ptr".
+Definition __IO_save_base : ident := $"_IO_save_base".
+Definition __IO_save_end : ident := $"_IO_save_end".
+Definition __IO_wide_data : ident := $"_IO_wide_data".
+Definition __IO_write_base : ident := $"_IO_write_base".
+Definition __IO_write_end : ident := $"_IO_write_end".
+Definition __IO_write_ptr : ident := $"_IO_write_ptr".
+Definition ___builtin_ais_annot : ident := $"__builtin_ais_annot".
+Definition ___builtin_annot : ident := $"__builtin_annot".
+Definition ___builtin_annot_intval : ident := $"__builtin_annot_intval".
+Definition ___builtin_bswap : ident := $"__builtin_bswap".
+Definition ___builtin_bswap16 : ident := $"__builtin_bswap16".
+Definition ___builtin_bswap32 : ident := $"__builtin_bswap32".
+Definition ___builtin_bswap64 : ident := $"__builtin_bswap64".
+Definition ___builtin_clz : ident := $"__builtin_clz".
+Definition ___builtin_clzl : ident := $"__builtin_clzl".
+Definition ___builtin_clzll : ident := $"__builtin_clzll".
+Definition ___builtin_ctz : ident := $"__builtin_ctz".
+Definition ___builtin_ctzl : ident := $"__builtin_ctzl".
+Definition ___builtin_ctzll : ident := $"__builtin_ctzll".
+Definition ___builtin_debug : ident := $"__builtin_debug".
+Definition ___builtin_expect : ident := $"__builtin_expect".
+Definition ___builtin_fabs : ident := $"__builtin_fabs".
+Definition ___builtin_fabsf : ident := $"__builtin_fabsf".
+Definition ___builtin_fmadd : ident := $"__builtin_fmadd".
+Definition ___builtin_fmax : ident := $"__builtin_fmax".
+Definition ___builtin_fmin : ident := $"__builtin_fmin".
+Definition ___builtin_fmsub : ident := $"__builtin_fmsub".
+Definition ___builtin_fnmadd : ident := $"__builtin_fnmadd".
+Definition ___builtin_fnmsub : ident := $"__builtin_fnmsub".
+Definition ___builtin_fsqrt : ident := $"__builtin_fsqrt".
+Definition ___builtin_membar : ident := $"__builtin_membar".
+Definition ___builtin_memcpy_aligned : ident := $"__builtin_memcpy_aligned".
+Definition ___builtin_read16_reversed : ident := $"__builtin_read16_reversed".
+Definition ___builtin_read32_reversed : ident := $"__builtin_read32_reversed".
+Definition ___builtin_sel : ident := $"__builtin_sel".
+Definition ___builtin_sqrt : ident := $"__builtin_sqrt".
+Definition ___builtin_unreachable : ident := $"__builtin_unreachable".
+Definition ___builtin_va_arg : ident := $"__builtin_va_arg".
+Definition ___builtin_va_copy : ident := $"__builtin_va_copy".
+Definition ___builtin_va_end : ident := $"__builtin_va_end".
+Definition ___builtin_va_start : ident := $"__builtin_va_start".
+Definition ___builtin_write16_reversed : ident := $"__builtin_write16_reversed".
+Definition ___builtin_write32_reversed : ident := $"__builtin_write32_reversed".
+Definition ___compcert_i64_dtos : ident := $"__compcert_i64_dtos".
+Definition ___compcert_i64_dtou : ident := $"__compcert_i64_dtou".
+Definition ___compcert_i64_sar : ident := $"__compcert_i64_sar".
+Definition ___compcert_i64_sdiv : ident := $"__compcert_i64_sdiv".
+Definition ___compcert_i64_shl : ident := $"__compcert_i64_shl".
+Definition ___compcert_i64_shr : ident := $"__compcert_i64_shr".
+Definition ___compcert_i64_smod : ident := $"__compcert_i64_smod".
+Definition ___compcert_i64_smulh : ident := $"__compcert_i64_smulh".
+Definition ___compcert_i64_stod : ident := $"__compcert_i64_stod".
+Definition ___compcert_i64_stof : ident := $"__compcert_i64_stof".
+Definition ___compcert_i64_udiv : ident := $"__compcert_i64_udiv".
+Definition ___compcert_i64_umod : ident := $"__compcert_i64_umod".
+Definition ___compcert_i64_umulh : ident := $"__compcert_i64_umulh".
+Definition ___compcert_i64_utod : ident := $"__compcert_i64_utod".
+Definition ___compcert_i64_utof : ident := $"__compcert_i64_utof".
+Definition ___compcert_va_composite : ident := $"__compcert_va_composite".
+Definition ___compcert_va_float64 : ident := $"__compcert_va_float64".
+Definition ___compcert_va_int32 : ident := $"__compcert_va_int32".
+Definition ___compcert_va_int64 : ident := $"__compcert_va_int64".
+Definition ___pad5 : ident := $"__pad5".
+Definition ___stringlit_1 : ident := $"__stringlit_1".
+Definition ___stringlit_2 : ident := $"__stringlit_2".
+Definition ___stringlit_3 : ident := $"__stringlit_3".
+Definition ___stringlit_4 : ident := $"__stringlit_4".
+Definition __chain : ident := $"_chain".
+Definition __codecvt : ident := $"_codecvt".
+Definition __cur_column : ident := $"_cur_column".
+Definition __fileno : ident := $"_fileno".
+Definition __flags : ident := $"_flags".
+Definition __flags2 : ident := $"_flags2".
+Definition __freeres_buf : ident := $"_freeres_buf".
+Definition __freeres_list : ident := $"_freeres_list".
+Definition __l : ident := $"_l".
+Definition __lock : ident := $"_lock".
+Definition __markers : ident := $"_markers".
+Definition __mode : ident := $"_mode".
+Definition __offset : ident := $"_offset".
+Definition __old_offset : ident := $"_old_offset".
+Definition __shortbuf : ident := $"_shortbuf".
+Definition __unused2 : ident := $"_unused2".
+Definition __vtable_offset : ident := $"_vtable_offset".
+Definition __wide_data : ident := $"_wide_data".
+Definition _a : ident := $"a".
+Definition _acquire : ident := $"acquire".
+Definition _append : ident := $"append".
+Definition _args : ident := $"args".
+Definition _atom_int : ident := $"atom_int".
+Definition _b : ident := $"b".
+Definition _buf : ident := $"buf".
+Definition _bufsize : ident := $"bufsize".
+Definition _c : ident := $"c".
+Definition _compute2 : ident := $"compute2".
+Definition _counter : ident := $"counter".
+Definition _ctr : ident := $"ctr".
+Definition _d : ident := $"d".
+Definition _data : ident := $"data".
+Definition _delete : ident := $"delete".
+Definition _des : ident := $"des".
+Definition _deserialize : ident := $"deserialize".
+Definition _dest_ctr : ident := $"dest_ctr".
+Definition _do_and : ident := $"do_and".
+Definition _do_or : ident := $"do_or".
+Definition _e : ident := $"e".
+Definition _exit : ident := $"exit".
+Definition _f : ident := $"f".
+Definition _foo : ident := $"foo".
+Definition _foo_methods : ident := $"foo_methods".
+Definition _foo_object : ident := $"foo_object".
+Definition _foo_reset : ident := $"foo_reset".
+Definition _foo_twiddle : ident := $"foo_twiddle".
+Definition _four : ident := $"four".
+Definition _fprintf : ident := $"fprintf".
+Definition _free : ident := $"free".
+Definition _freeN : ident := $"freeN".
+Definition _freelock : ident := $"freelock".
+Definition _g : ident := $"g".
+Definition _get : ident := $"get".
+Definition _getchar : ident := $"getchar".
+Definition _getchar_blocking : ident := $"getchar_blocking".
+Definition _getchars : ident := $"getchars".
+Definition _h : ident := $"h".
+Definition _head : ident := $"head".
+Definition _hi : ident := $"hi".
+Definition _i : ident := $"i".
+Definition _i__1 : ident := $"i__1".
+Definition _incr : ident := $"incr".
+Definition _init_ctr : ident := $"init_ctr".
+Definition _insert : ident := $"insert".
+Definition _intpair : ident := $"intpair".
+Definition _intpair_deserialize : ident := $"intpair_deserialize".
+Definition _intpair_message : ident := $"intpair_message".
+Definition _intpair_serialize : ident := $"intpair_serialize".
+Definition _j : ident := $"j".
+Definition _k : ident := $"k".
+Definition _key : ident := $"key".
+Definition _l : ident := $"l".
+Definition _left : ident := $"left".
+Definition _len : ident := $"len".
+Definition _length : ident := $"length".
+Definition _list : ident := $"list".
+Definition _lo : ident := $"lo".
+Definition _lock : ident := $"lock".
+Definition _lookup : ident := $"lookup".
+Definition _main : ident := $"main".
+Definition _make_foo : ident := $"make_foo".
+Definition _makelock : ident := $"makelock".
+Definition _malloc : ident := $"malloc".
+Definition _mallocN : ident := $"mallocN".
+Definition _message : ident := $"message".
+Definition _methods : ident := $"methods".
+Definition _mid : ident := $"mid".
+Definition _min : ident := $"min".
+Definition _minimum : ident := $"minimum".
+Definition _mtable : ident := $"mtable".
+Definition _multi_command : ident := $"multi_command".
+Definition _multi_command_s : ident := $"multi_command_s".
+Definition _n : ident := $"n".
+Definition _object : ident := $"object".
+Definition _p : ident := $"p".
+Definition _p0 : ident := $"p0".
+Definition _p1 : ident := $"p1".
+Definition _p2 : ident := $"p2".
+Definition _p3 : ident := $"p3".
+Definition _p4 : ident := $"p4".
+Definition _p5 : ident := $"p5".
+Definition _p6 : ident := $"p6".
+Definition _p7 : ident := $"p7".
+Definition _p_reset : ident := $"p_reset".
+Definition _p_twiddle : ident := $"p_twiddle".
+Definition _pa : ident := $"pa".
+Definition _pb : ident := $"pb".
+Definition _print_int : ident := $"print_int".
+Definition _print_intr : ident := $"print_intr".
+Definition _printf : ident := $"printf".
+Definition _pushdown_left : ident := $"pushdown_left".
+Definition _putchar : ident := $"putchar".
+Definition _putchar_blocking : ident := $"putchar_blocking".
+Definition _putchars : ident := $"putchars".
+Definition _q : ident := $"q".
+Definition _r : ident := $"r".
+Definition _read : ident := $"read".
+Definition _release : ident := $"release".
+Definition _reset : ident := $"reset".
+Definition _right : ident := $"right".
+Definition _s : ident := $"s".
+Definition _search : ident := $"search".
+Definition _self : ident := $"self".
+Definition _ser : ident := $"ser".
+Definition _serialize : ident := $"serialize".
+Definition _set : ident := $"set".
+Definition _spawn : ident := $"spawn".
+Definition _stdout : ident := $"stdout".
+Definition _sub1 : ident := $"sub1".
+Definition _sub2 : ident := $"sub2".
+Definition _sub3 : ident := $"sub3".
+Definition _t : ident := $"t".
+Definition _tail : ident := $"tail".
+Definition _tgt : ident := $"tgt".
+Definition _thread_func : ident := $"thread_func".
+Definition _thread_lock : ident := $"thread_lock".
+Definition _tree : ident := $"tree".
+Definition _tree_free : ident := $"tree_free".
+Definition _treebox_free : ident := $"treebox_free".
+Definition _treebox_new : ident := $"treebox_new".
+Definition _turn_left : ident := $"turn_left".
+Definition _twiddle : ident := $"twiddle".
+Definition _u : ident := $"u".
+Definition _v : ident := $"v".
+Definition _val : ident := $"val".
+Definition _value : ident := $"value".
+Definition _x : ident := $"x".
+Definition _x1 : ident := $"x1".
+Definition _x2 : ident := $"x2".
+Definition _y : ident := $"y".
+Definition _y1 : ident := $"y1".
+Definition _y2 : ident := $"y2".
+Definition _z : ident := $"z".
+Definition _z1 : ident := $"z1".
+Definition _z2 : ident := $"z2".
+Definition _t'1 : ident := 128%positive.
 
 Definition v___stringlit_3 := {|
   gvar_info := (tarray tschar 16);
@@ -236,471 +289,346 @@ Definition v___stringlit_1 := {|
   gvar_volatile := false
 |}.
 
+Definition v_stdout := {|
+  gvar_info := (tptr (Tstruct __IO_FILE noattr));
+  gvar_init := nil;
+  gvar_readonly := false;
+  gvar_volatile := false
+|}.
+
 Definition f_main := {|
   fn_return := tint;
   fn_callconv := cc_default;
   fn_params := nil;
   fn_vars := nil;
-  fn_temps := ((_t'1, (tptr (Tstruct __reent noattr))) ::
-               (_t'2, (tptr (Tstruct ___sFILE64 noattr))) :: nil);
+  fn_temps := ((_t'1, (tptr (Tstruct __IO_FILE noattr))) :: nil);
   fn_body :=
 (Ssequence
   (Ssequence
     (Scall None
-      (Evar _printf (Tfunction (Tcons (tptr tschar) Tnil) tint
+      (Evar _printf (Tfunction ((tptr tschar) :: nil) tint
                       {|cc_vararg:=(Some 1); cc_unproto:=false; cc_structret:=false|}))
       ((Evar ___stringlit_1 (tarray tschar 15)) :: nil))
     (Ssequence
       (Ssequence
-        (Scall (Some _t'1)
-          (Evar ___getreent (Tfunction Tnil (tptr (Tstruct __reent noattr))
-                              cc_default)) nil)
-        (Ssequence
-          (Sset _t'2
-            (Efield
-              (Ederef (Etempvar _t'1 (tptr (Tstruct __reent noattr)))
-                (Tstruct __reent noattr)) __stdout
-              (tptr (Tstruct ___sFILE64 noattr))))
-          (Scall None
-            (Evar _fprintf (Tfunction
-                             (Tcons (tptr (Tstruct ___sFILE64 noattr))
-                               (Tcons (tptr tschar) Tnil)) tint
-                             {|cc_vararg:=(Some 2); cc_unproto:=false; cc_structret:=false|}))
-            ((Etempvar _t'2 (tptr (Tstruct ___sFILE64 noattr))) ::
-             (Evar ___stringlit_3 (tarray tschar 16)) ::
-             (Evar ___stringlit_2 (tarray tschar 5)) ::
-             (Econst_int (Int.repr 2) tint) :: nil))))
+        (Sset _t'1 (Evar _stdout (tptr (Tstruct __IO_FILE noattr))))
+        (Scall None
+          (Evar _fprintf (Tfunction
+                           ((tptr (Tstruct __IO_FILE noattr)) ::
+                            (tptr tschar) :: nil) tint
+                           {|cc_vararg:=(Some 2); cc_unproto:=false; cc_structret:=false|}))
+          ((Etempvar _t'1 (tptr (Tstruct __IO_FILE noattr))) ::
+           (Evar ___stringlit_3 (tarray tschar 16)) ::
+           (Evar ___stringlit_2 (tarray tschar 5)) ::
+           (Econst_int (Int.repr 2) tint) :: nil)))
       (Sreturn (Some (Econst_int (Int.repr 0) tint)))))
   (Sreturn (Some (Econst_int (Int.repr 0) tint))))
 |}.
 
 Definition composites : list composite_definition :=
-(Composite __140 Union
-   (Member_plain ___wch tuint :: Member_plain ___wchb (tarray tuchar 4) ::
+(Composite __IO_FILE Struct
+   (Member_plain __flags tint :: Member_plain __IO_read_ptr (tptr tschar) ::
+    Member_plain __IO_read_end (tptr tschar) ::
+    Member_plain __IO_read_base (tptr tschar) ::
+    Member_plain __IO_write_base (tptr tschar) ::
+    Member_plain __IO_write_ptr (tptr tschar) ::
+    Member_plain __IO_write_end (tptr tschar) ::
+    Member_plain __IO_buf_base (tptr tschar) ::
+    Member_plain __IO_buf_end (tptr tschar) ::
+    Member_plain __IO_save_base (tptr tschar) ::
+    Member_plain __IO_backup_base (tptr tschar) ::
+    Member_plain __IO_save_end (tptr tschar) ::
+    Member_plain __markers (tptr (Tstruct __IO_marker noattr)) ::
+    Member_plain __chain (tptr (Tstruct __IO_FILE noattr)) ::
+    Member_plain __fileno tint :: Member_plain __flags2 tint ::
+    Member_plain __old_offset tlong :: Member_plain __cur_column tushort ::
+    Member_plain __vtable_offset tschar ::
+    Member_plain __shortbuf (tarray tschar 1) ::
+    Member_plain __lock (tptr tvoid) :: Member_plain __offset tlong ::
+    Member_plain __codecvt (tptr (Tstruct __IO_codecvt noattr)) ::
+    Member_plain __wide_data (tptr (Tstruct __IO_wide_data noattr)) ::
+    Member_plain __freeres_list (tptr (Tstruct __IO_FILE noattr)) ::
+    Member_plain __freeres_buf (tptr tvoid) :: Member_plain ___pad5 tulong ::
+    Member_plain __mode tint :: Member_plain __unused2 (tarray tschar 20) ::
     nil)
-   noattr ::
- Composite __139 Struct
-   (Member_plain ___count tint ::
-    Member_plain ___value (Tunion __140 noattr) :: nil)
-   noattr ::
- Composite __Bigint Struct
-   (Member_plain __next (tptr (Tstruct __Bigint noattr)) ::
-    Member_plain __k tint :: Member_plain __maxwds tint ::
-    Member_plain __sign tint :: Member_plain __wds tint ::
-    Member_plain __x (tarray tuint 1) :: nil)
-   noattr ::
- Composite ___tm Struct
-   (Member_plain ___tm_sec tint :: Member_plain ___tm_min tint ::
-    Member_plain ___tm_hour tint :: Member_plain ___tm_mday tint ::
-    Member_plain ___tm_mon tint :: Member_plain ___tm_year tint ::
-    Member_plain ___tm_wday tint :: Member_plain ___tm_yday tint ::
-    Member_plain ___tm_isdst tint :: nil)
-   noattr ::
- Composite __on_exit_args Struct
-   (Member_plain __fnargs (tarray (tptr tvoid) 32) ::
-    Member_plain __dso_handle (tarray (tptr tvoid) 32) ::
-    Member_plain __fntypes tuint :: Member_plain __is_cxa tuint :: nil)
-   noattr ::
- Composite __atexit Struct
-   (Member_plain __next (tptr (Tstruct __atexit noattr)) ::
-    Member_plain __ind tint ::
-    Member_plain __fns (tarray (tptr (Tfunction Tnil tvoid cc_default)) 32) ::
-    Member_plain __on_exit_args (Tstruct __on_exit_args noattr) :: nil)
-   noattr ::
- Composite ___sbuf Struct
-   (Member_plain __base (tptr tuchar) :: Member_plain __size tint :: nil)
-   noattr ::
- Composite ___sFILE64 Struct
-   (Member_plain __p (tptr tuchar) :: Member_plain __r tint ::
-    Member_plain __w tint :: Member_plain __flags tshort ::
-    Member_plain __file tshort ::
-    Member_plain __bf (Tstruct ___sbuf noattr) ::
-    Member_plain __lbfsize tint ::
-    Member_plain __data (tptr (Tstruct __reent noattr)) ::
-    Member_plain __cookie (tptr tvoid) ::
-    Member_plain __read
-      (tptr (Tfunction
-              (Tcons (tptr (Tstruct __reent noattr))
-                (Tcons (tptr tvoid)
-                  (Tcons (tptr tschar) (Tcons tulong Tnil)))) tlong
-              cc_default)) ::
-    Member_plain __write
-      (tptr (Tfunction
-              (Tcons (tptr (Tstruct __reent noattr))
-                (Tcons (tptr tvoid)
-                  (Tcons (tptr tschar) (Tcons tulong Tnil)))) tlong
-              cc_default)) ::
-    Member_plain __seek
-      (tptr (Tfunction
-              (Tcons (tptr (Tstruct __reent noattr))
-                (Tcons (tptr tvoid) (Tcons tlong (Tcons tint Tnil)))) tlong
-              cc_default)) ::
-    Member_plain __close
-      (tptr (Tfunction
-              (Tcons (tptr (Tstruct __reent noattr))
-                (Tcons (tptr tvoid) Tnil)) tint cc_default)) ::
-    Member_plain __ub (Tstruct ___sbuf noattr) ::
-    Member_plain __up (tptr tuchar) :: Member_plain __ur tint ::
-    Member_plain __ubuf (tarray tuchar 3) ::
-    Member_plain __nbuf (tarray tuchar 1) ::
-    Member_plain __lb (Tstruct ___sbuf noattr) ::
-    Member_plain __blksize tint :: Member_plain __flags2 tint ::
-    Member_plain __offset tlong ::
-    Member_plain __seek64
-      (tptr (Tfunction
-              (Tcons (tptr (Tstruct __reent noattr))
-                (Tcons (tptr tvoid) (Tcons tlong (Tcons tint Tnil)))) tlong
-              cc_default)) :: Member_plain __lock (tptr tvoid) ::
-    Member_plain __mbstate (Tstruct __139 noattr) :: nil)
-   noattr ::
- Composite __glue Struct
-   (Member_plain __next (tptr (Tstruct __glue noattr)) ::
-    Member_plain __niobs tint ::
-    Member_plain __iobs (tptr (Tstruct ___sFILE64 noattr)) :: nil)
-   noattr ::
- Composite __rand48 Struct
-   (Member_plain __seed (tarray tushort 3) ::
-    Member_plain __mult (tarray tushort 3) :: Member_plain __add tushort ::
-    nil)
-   noattr ::
- Composite __214 Struct
-   (Member_plain __unused_rand tuint ::
-    Member_plain __strtok_last (tptr tschar) ::
-    Member_plain __asctime_buf (tarray tschar 26) ::
-    Member_plain __localtime_buf (Tstruct ___tm noattr) ::
-    Member_plain __gamma_signgam tint :: Member_plain __rand_next tulong ::
-    Member_plain __r48 (Tstruct __rand48 noattr) ::
-    Member_plain __mblen_state (Tstruct __139 noattr) ::
-    Member_plain __mbtowc_state (Tstruct __139 noattr) ::
-    Member_plain __wctomb_state (Tstruct __139 noattr) ::
-    Member_plain __l64a_buf (tarray tschar 8) ::
-    Member_plain __signal_buf (tarray tschar 24) ::
-    Member_plain __getdate_err tint ::
-    Member_plain __mbrlen_state (Tstruct __139 noattr) ::
-    Member_plain __mbrtowc_state (Tstruct __139 noattr) ::
-    Member_plain __mbsrtowcs_state (Tstruct __139 noattr) ::
-    Member_plain __wcrtomb_state (Tstruct __139 noattr) ::
-    Member_plain __wcsrtombs_state (Tstruct __139 noattr) ::
-    Member_plain __h_errno tint :: nil)
-   noattr ::
- Composite __215 Struct
-   (Member_plain __nextf (tarray (tptr tuchar) 30) ::
-    Member_plain __nmalloc (tarray tuint 30) :: nil)
-   noattr ::
- Composite __213 Union
-   (Member_plain __reent (Tstruct __214 noattr) ::
-    Member_plain __unused (Tstruct __215 noattr) :: nil)
-   noattr ::
- Composite __reent Struct
-   (Member_plain __errno tint ::
-    Member_plain __stdin (tptr (Tstruct ___sFILE64 noattr)) ::
-    Member_plain __stdout (tptr (Tstruct ___sFILE64 noattr)) ::
-    Member_plain __stderr (tptr (Tstruct ___sFILE64 noattr)) ::
-    Member_plain __inc tint :: Member_plain __emergency (tarray tschar 25) ::
-    Member_plain __unspecified_locale_info tint ::
-    Member_plain __locale (tptr (Tstruct ___locale_t noattr)) ::
-    Member_plain ___sdidinit tint ::
-    Member_plain ___cleanup
-      (tptr (Tfunction (Tcons (tptr (Tstruct __reent noattr)) Tnil) tvoid
-              cc_default)) ::
-    Member_plain __result (tptr (Tstruct __Bigint noattr)) ::
-    Member_plain __result_k tint ::
-    Member_plain __p5s (tptr (Tstruct __Bigint noattr)) ::
-    Member_plain __freelist (tptr (tptr (Tstruct __Bigint noattr))) ::
-    Member_plain __cvtlen tint :: Member_plain __cvtbuf (tptr tschar) ::
-    Member_plain __new (Tunion __213 noattr) ::
-    Member_plain __atexit (tptr (Tstruct __atexit noattr)) ::
-    Member_plain __atexit0 (Tstruct __atexit noattr) ::
-    Member_plain __sig_func
-      (tptr (tptr (Tfunction (Tcons tint Tnil) tvoid cc_default))) ::
-    Member_plain ___sglue (Tstruct __glue noattr) ::
-    Member_plain ___sf (tarray (Tstruct ___sFILE64 noattr) 3) :: nil)
    noattr :: nil).
 
 Definition global_definitions : list (ident * globdef fundef type) :=
 ((___compcert_va_int32,
    Gfun(External (EF_runtime "__compcert_va_int32"
-                   (mksignature (AST.Tlong :: nil) AST.Tint cc_default))
-     (Tcons (tptr tvoid) Tnil) tuint cc_default)) ::
+                   (mksignature (AST.Xptr :: nil) AST.Xint cc_default))
+     ((tptr tvoid) :: nil) tuint cc_default)) ::
  (___compcert_va_int64,
    Gfun(External (EF_runtime "__compcert_va_int64"
-                   (mksignature (AST.Tlong :: nil) AST.Tlong cc_default))
-     (Tcons (tptr tvoid) Tnil) tulong cc_default)) ::
+                   (mksignature (AST.Xptr :: nil) AST.Xlong cc_default))
+     ((tptr tvoid) :: nil) tulong cc_default)) ::
  (___compcert_va_float64,
    Gfun(External (EF_runtime "__compcert_va_float64"
-                   (mksignature (AST.Tlong :: nil) AST.Tfloat cc_default))
-     (Tcons (tptr tvoid) Tnil) tdouble cc_default)) ::
+                   (mksignature (AST.Xptr :: nil) AST.Xfloat cc_default))
+     ((tptr tvoid) :: nil) tdouble cc_default)) ::
  (___compcert_va_composite,
    Gfun(External (EF_runtime "__compcert_va_composite"
-                   (mksignature (AST.Tlong :: AST.Tlong :: nil) AST.Tlong
-                     cc_default)) (Tcons (tptr tvoid) (Tcons tulong Tnil))
+                   (mksignature (AST.Xptr :: AST.Xlong :: nil) AST.Xptr
+                     cc_default)) ((tptr tvoid) :: tulong :: nil)
      (tptr tvoid) cc_default)) ::
  (___compcert_i64_dtos,
    Gfun(External (EF_runtime "__compcert_i64_dtos"
-                   (mksignature (AST.Tfloat :: nil) AST.Tlong cc_default))
-     (Tcons tdouble Tnil) tlong cc_default)) ::
+                   (mksignature (AST.Xfloat :: nil) AST.Xlong cc_default))
+     (tdouble :: nil) tlong cc_default)) ::
  (___compcert_i64_dtou,
    Gfun(External (EF_runtime "__compcert_i64_dtou"
-                   (mksignature (AST.Tfloat :: nil) AST.Tlong cc_default))
-     (Tcons tdouble Tnil) tulong cc_default)) ::
+                   (mksignature (AST.Xfloat :: nil) AST.Xlong cc_default))
+     (tdouble :: nil) tulong cc_default)) ::
  (___compcert_i64_stod,
    Gfun(External (EF_runtime "__compcert_i64_stod"
-                   (mksignature (AST.Tlong :: nil) AST.Tfloat cc_default))
-     (Tcons tlong Tnil) tdouble cc_default)) ::
+                   (mksignature (AST.Xlong :: nil) AST.Xfloat cc_default))
+     (tlong :: nil) tdouble cc_default)) ::
  (___compcert_i64_utod,
    Gfun(External (EF_runtime "__compcert_i64_utod"
-                   (mksignature (AST.Tlong :: nil) AST.Tfloat cc_default))
-     (Tcons tulong Tnil) tdouble cc_default)) ::
+                   (mksignature (AST.Xlong :: nil) AST.Xfloat cc_default))
+     (tulong :: nil) tdouble cc_default)) ::
  (___compcert_i64_stof,
    Gfun(External (EF_runtime "__compcert_i64_stof"
-                   (mksignature (AST.Tlong :: nil) AST.Tsingle cc_default))
-     (Tcons tlong Tnil) tfloat cc_default)) ::
+                   (mksignature (AST.Xlong :: nil) AST.Xsingle cc_default))
+     (tlong :: nil) tfloat cc_default)) ::
  (___compcert_i64_utof,
    Gfun(External (EF_runtime "__compcert_i64_utof"
-                   (mksignature (AST.Tlong :: nil) AST.Tsingle cc_default))
-     (Tcons tulong Tnil) tfloat cc_default)) ::
+                   (mksignature (AST.Xlong :: nil) AST.Xsingle cc_default))
+     (tulong :: nil) tfloat cc_default)) ::
  (___compcert_i64_sdiv,
    Gfun(External (EF_runtime "__compcert_i64_sdiv"
-                   (mksignature (AST.Tlong :: AST.Tlong :: nil) AST.Tlong
-                     cc_default)) (Tcons tlong (Tcons tlong Tnil)) tlong
-     cc_default)) ::
+                   (mksignature (AST.Xlong :: AST.Xlong :: nil) AST.Xlong
+                     cc_default)) (tlong :: tlong :: nil) tlong cc_default)) ::
  (___compcert_i64_udiv,
    Gfun(External (EF_runtime "__compcert_i64_udiv"
-                   (mksignature (AST.Tlong :: AST.Tlong :: nil) AST.Tlong
-                     cc_default)) (Tcons tulong (Tcons tulong Tnil)) tulong
+                   (mksignature (AST.Xlong :: AST.Xlong :: nil) AST.Xlong
+                     cc_default)) (tulong :: tulong :: nil) tulong
      cc_default)) ::
  (___compcert_i64_smod,
    Gfun(External (EF_runtime "__compcert_i64_smod"
-                   (mksignature (AST.Tlong :: AST.Tlong :: nil) AST.Tlong
-                     cc_default)) (Tcons tlong (Tcons tlong Tnil)) tlong
-     cc_default)) ::
+                   (mksignature (AST.Xlong :: AST.Xlong :: nil) AST.Xlong
+                     cc_default)) (tlong :: tlong :: nil) tlong cc_default)) ::
  (___compcert_i64_umod,
    Gfun(External (EF_runtime "__compcert_i64_umod"
-                   (mksignature (AST.Tlong :: AST.Tlong :: nil) AST.Tlong
-                     cc_default)) (Tcons tulong (Tcons tulong Tnil)) tulong
+                   (mksignature (AST.Xlong :: AST.Xlong :: nil) AST.Xlong
+                     cc_default)) (tulong :: tulong :: nil) tulong
      cc_default)) ::
  (___compcert_i64_shl,
    Gfun(External (EF_runtime "__compcert_i64_shl"
-                   (mksignature (AST.Tlong :: AST.Tint :: nil) AST.Tlong
-                     cc_default)) (Tcons tlong (Tcons tint Tnil)) tlong
-     cc_default)) ::
+                   (mksignature (AST.Xlong :: AST.Xint :: nil) AST.Xlong
+                     cc_default)) (tlong :: tint :: nil) tlong cc_default)) ::
  (___compcert_i64_shr,
    Gfun(External (EF_runtime "__compcert_i64_shr"
-                   (mksignature (AST.Tlong :: AST.Tint :: nil) AST.Tlong
-                     cc_default)) (Tcons tulong (Tcons tint Tnil)) tulong
-     cc_default)) ::
+                   (mksignature (AST.Xlong :: AST.Xint :: nil) AST.Xlong
+                     cc_default)) (tulong :: tint :: nil) tulong cc_default)) ::
  (___compcert_i64_sar,
    Gfun(External (EF_runtime "__compcert_i64_sar"
-                   (mksignature (AST.Tlong :: AST.Tint :: nil) AST.Tlong
-                     cc_default)) (Tcons tlong (Tcons tint Tnil)) tlong
-     cc_default)) ::
+                   (mksignature (AST.Xlong :: AST.Xint :: nil) AST.Xlong
+                     cc_default)) (tlong :: tint :: nil) tlong cc_default)) ::
  (___compcert_i64_smulh,
    Gfun(External (EF_runtime "__compcert_i64_smulh"
-                   (mksignature (AST.Tlong :: AST.Tlong :: nil) AST.Tlong
-                     cc_default)) (Tcons tlong (Tcons tlong Tnil)) tlong
-     cc_default)) ::
+                   (mksignature (AST.Xlong :: AST.Xlong :: nil) AST.Xlong
+                     cc_default)) (tlong :: tlong :: nil) tlong cc_default)) ::
  (___compcert_i64_umulh,
    Gfun(External (EF_runtime "__compcert_i64_umulh"
-                   (mksignature (AST.Tlong :: AST.Tlong :: nil) AST.Tlong
-                     cc_default)) (Tcons tulong (Tcons tulong Tnil)) tulong
+                   (mksignature (AST.Xlong :: AST.Xlong :: nil) AST.Xlong
+                     cc_default)) (tulong :: tulong :: nil) tulong
      cc_default)) :: (___stringlit_3, Gvar v___stringlit_3) ::
  (___stringlit_2, Gvar v___stringlit_2) ::
  (___stringlit_1, Gvar v___stringlit_1) ::
+ (___builtin_ais_annot,
+   Gfun(External (EF_builtin "__builtin_ais_annot"
+                   (mksignature (AST.Xptr :: nil) AST.Xvoid
+                     {|cc_vararg:=(Some 1); cc_unproto:=false; cc_structret:=false|}))
+     ((tptr tschar) :: nil) tvoid
+     {|cc_vararg:=(Some 1); cc_unproto:=false; cc_structret:=false|})) ::
  (___builtin_bswap64,
    Gfun(External (EF_builtin "__builtin_bswap64"
-                   (mksignature (AST.Tlong :: nil) AST.Tlong cc_default))
-     (Tcons tulong Tnil) tulong cc_default)) ::
+                   (mksignature (AST.Xlong :: nil) AST.Xlong cc_default))
+     (tulong :: nil) tulong cc_default)) ::
  (___builtin_bswap,
    Gfun(External (EF_builtin "__builtin_bswap"
-                   (mksignature (AST.Tint :: nil) AST.Tint cc_default))
-     (Tcons tuint Tnil) tuint cc_default)) ::
+                   (mksignature (AST.Xint :: nil) AST.Xint cc_default))
+     (tuint :: nil) tuint cc_default)) ::
  (___builtin_bswap32,
    Gfun(External (EF_builtin "__builtin_bswap32"
-                   (mksignature (AST.Tint :: nil) AST.Tint cc_default))
-     (Tcons tuint Tnil) tuint cc_default)) ::
+                   (mksignature (AST.Xint :: nil) AST.Xint cc_default))
+     (tuint :: nil) tuint cc_default)) ::
  (___builtin_bswap16,
    Gfun(External (EF_builtin "__builtin_bswap16"
-                   (mksignature (AST.Tint :: nil) AST.Tint16unsigned
-                     cc_default)) (Tcons tushort Tnil) tushort cc_default)) ::
+                   (mksignature (AST.Xint16unsigned :: nil)
+                     AST.Xint16unsigned cc_default)) (tushort :: nil) tushort
+     cc_default)) ::
  (___builtin_clz,
    Gfun(External (EF_builtin "__builtin_clz"
-                   (mksignature (AST.Tint :: nil) AST.Tint cc_default))
-     (Tcons tuint Tnil) tint cc_default)) ::
+                   (mksignature (AST.Xint :: nil) AST.Xint cc_default))
+     (tuint :: nil) tint cc_default)) ::
  (___builtin_clzl,
    Gfun(External (EF_builtin "__builtin_clzl"
-                   (mksignature (AST.Tlong :: nil) AST.Tint cc_default))
-     (Tcons tulong Tnil) tint cc_default)) ::
+                   (mksignature (AST.Xlong :: nil) AST.Xint cc_default))
+     (tulong :: nil) tint cc_default)) ::
  (___builtin_clzll,
    Gfun(External (EF_builtin "__builtin_clzll"
-                   (mksignature (AST.Tlong :: nil) AST.Tint cc_default))
-     (Tcons tulong Tnil) tint cc_default)) ::
+                   (mksignature (AST.Xlong :: nil) AST.Xint cc_default))
+     (tulong :: nil) tint cc_default)) ::
  (___builtin_ctz,
    Gfun(External (EF_builtin "__builtin_ctz"
-                   (mksignature (AST.Tint :: nil) AST.Tint cc_default))
-     (Tcons tuint Tnil) tint cc_default)) ::
+                   (mksignature (AST.Xint :: nil) AST.Xint cc_default))
+     (tuint :: nil) tint cc_default)) ::
  (___builtin_ctzl,
    Gfun(External (EF_builtin "__builtin_ctzl"
-                   (mksignature (AST.Tlong :: nil) AST.Tint cc_default))
-     (Tcons tulong Tnil) tint cc_default)) ::
+                   (mksignature (AST.Xlong :: nil) AST.Xint cc_default))
+     (tulong :: nil) tint cc_default)) ::
  (___builtin_ctzll,
    Gfun(External (EF_builtin "__builtin_ctzll"
-                   (mksignature (AST.Tlong :: nil) AST.Tint cc_default))
-     (Tcons tulong Tnil) tint cc_default)) ::
+                   (mksignature (AST.Xlong :: nil) AST.Xint cc_default))
+     (tulong :: nil) tint cc_default)) ::
  (___builtin_fabs,
    Gfun(External (EF_builtin "__builtin_fabs"
-                   (mksignature (AST.Tfloat :: nil) AST.Tfloat cc_default))
-     (Tcons tdouble Tnil) tdouble cc_default)) ::
+                   (mksignature (AST.Xfloat :: nil) AST.Xfloat cc_default))
+     (tdouble :: nil) tdouble cc_default)) ::
  (___builtin_fabsf,
    Gfun(External (EF_builtin "__builtin_fabsf"
-                   (mksignature (AST.Tsingle :: nil) AST.Tsingle cc_default))
-     (Tcons tfloat Tnil) tfloat cc_default)) ::
+                   (mksignature (AST.Xsingle :: nil) AST.Xsingle cc_default))
+     (tfloat :: nil) tfloat cc_default)) ::
  (___builtin_fsqrt,
    Gfun(External (EF_builtin "__builtin_fsqrt"
-                   (mksignature (AST.Tfloat :: nil) AST.Tfloat cc_default))
-     (Tcons tdouble Tnil) tdouble cc_default)) ::
+                   (mksignature (AST.Xfloat :: nil) AST.Xfloat cc_default))
+     (tdouble :: nil) tdouble cc_default)) ::
  (___builtin_sqrt,
    Gfun(External (EF_builtin "__builtin_sqrt"
-                   (mksignature (AST.Tfloat :: nil) AST.Tfloat cc_default))
-     (Tcons tdouble Tnil) tdouble cc_default)) ::
+                   (mksignature (AST.Xfloat :: nil) AST.Xfloat cc_default))
+     (tdouble :: nil) tdouble cc_default)) ::
  (___builtin_memcpy_aligned,
    Gfun(External (EF_builtin "__builtin_memcpy_aligned"
                    (mksignature
-                     (AST.Tlong :: AST.Tlong :: AST.Tlong :: AST.Tlong ::
-                      nil) AST.Tvoid cc_default))
-     (Tcons (tptr tvoid)
-       (Tcons (tptr tvoid) (Tcons tulong (Tcons tulong Tnil)))) tvoid
+                     (AST.Xptr :: AST.Xptr :: AST.Xlong :: AST.Xlong :: nil)
+                     AST.Xvoid cc_default))
+     ((tptr tvoid) :: (tptr tvoid) :: tulong :: tulong :: nil) tvoid
      cc_default)) ::
  (___builtin_sel,
    Gfun(External (EF_builtin "__builtin_sel"
-                   (mksignature (AST.Tint :: nil) AST.Tvoid
+                   (mksignature (AST.Xbool :: nil) AST.Xvoid
                      {|cc_vararg:=(Some 1); cc_unproto:=false; cc_structret:=false|}))
-     (Tcons tbool Tnil) tvoid
+     (tbool :: nil) tvoid
      {|cc_vararg:=(Some 1); cc_unproto:=false; cc_structret:=false|})) ::
  (___builtin_annot,
    Gfun(External (EF_builtin "__builtin_annot"
-                   (mksignature (AST.Tlong :: nil) AST.Tvoid
+                   (mksignature (AST.Xptr :: nil) AST.Xvoid
                      {|cc_vararg:=(Some 1); cc_unproto:=false; cc_structret:=false|}))
-     (Tcons (tptr tschar) Tnil) tvoid
+     ((tptr tschar) :: nil) tvoid
      {|cc_vararg:=(Some 1); cc_unproto:=false; cc_structret:=false|})) ::
  (___builtin_annot_intval,
    Gfun(External (EF_builtin "__builtin_annot_intval"
-                   (mksignature (AST.Tlong :: AST.Tint :: nil) AST.Tint
-                     cc_default)) (Tcons (tptr tschar) (Tcons tint Tnil))
-     tint cc_default)) ::
+                   (mksignature (AST.Xptr :: AST.Xint :: nil) AST.Xint
+                     cc_default)) ((tptr tschar) :: tint :: nil) tint
+     cc_default)) ::
  (___builtin_membar,
    Gfun(External (EF_builtin "__builtin_membar"
-                   (mksignature nil AST.Tvoid cc_default)) Tnil tvoid
+                   (mksignature nil AST.Xvoid cc_default)) nil tvoid
      cc_default)) ::
  (___builtin_va_start,
    Gfun(External (EF_builtin "__builtin_va_start"
-                   (mksignature (AST.Tlong :: nil) AST.Tvoid cc_default))
-     (Tcons (tptr tvoid) Tnil) tvoid cc_default)) ::
+                   (mksignature (AST.Xptr :: nil) AST.Xvoid cc_default))
+     ((tptr tvoid) :: nil) tvoid cc_default)) ::
  (___builtin_va_arg,
    Gfun(External (EF_builtin "__builtin_va_arg"
-                   (mksignature (AST.Tlong :: AST.Tint :: nil) AST.Tvoid
-                     cc_default)) (Tcons (tptr tvoid) (Tcons tuint Tnil))
-     tvoid cc_default)) ::
+                   (mksignature (AST.Xptr :: AST.Xint :: nil) AST.Xvoid
+                     cc_default)) ((tptr tvoid) :: tuint :: nil) tvoid
+     cc_default)) ::
  (___builtin_va_copy,
    Gfun(External (EF_builtin "__builtin_va_copy"
-                   (mksignature (AST.Tlong :: AST.Tlong :: nil) AST.Tvoid
-                     cc_default))
-     (Tcons (tptr tvoid) (Tcons (tptr tvoid) Tnil)) tvoid cc_default)) ::
+                   (mksignature (AST.Xptr :: AST.Xptr :: nil) AST.Xvoid
+                     cc_default)) ((tptr tvoid) :: (tptr tvoid) :: nil) tvoid
+     cc_default)) ::
  (___builtin_va_end,
    Gfun(External (EF_builtin "__builtin_va_end"
-                   (mksignature (AST.Tlong :: nil) AST.Tvoid cc_default))
-     (Tcons (tptr tvoid) Tnil) tvoid cc_default)) ::
+                   (mksignature (AST.Xptr :: nil) AST.Xvoid cc_default))
+     ((tptr tvoid) :: nil) tvoid cc_default)) ::
  (___builtin_unreachable,
    Gfun(External (EF_builtin "__builtin_unreachable"
-                   (mksignature nil AST.Tvoid cc_default)) Tnil tvoid
+                   (mksignature nil AST.Xvoid cc_default)) nil tvoid
      cc_default)) ::
  (___builtin_expect,
    Gfun(External (EF_builtin "__builtin_expect"
-                   (mksignature (AST.Tlong :: AST.Tlong :: nil) AST.Tlong
-                     cc_default)) (Tcons tlong (Tcons tlong Tnil)) tlong
-     cc_default)) ::
+                   (mksignature (AST.Xlong :: AST.Xlong :: nil) AST.Xlong
+                     cc_default)) (tlong :: tlong :: nil) tlong cc_default)) ::
  (___builtin_fmax,
    Gfun(External (EF_builtin "__builtin_fmax"
-                   (mksignature (AST.Tfloat :: AST.Tfloat :: nil) AST.Tfloat
-                     cc_default)) (Tcons tdouble (Tcons tdouble Tnil))
-     tdouble cc_default)) ::
+                   (mksignature (AST.Xfloat :: AST.Xfloat :: nil) AST.Xfloat
+                     cc_default)) (tdouble :: tdouble :: nil) tdouble
+     cc_default)) ::
  (___builtin_fmin,
    Gfun(External (EF_builtin "__builtin_fmin"
-                   (mksignature (AST.Tfloat :: AST.Tfloat :: nil) AST.Tfloat
-                     cc_default)) (Tcons tdouble (Tcons tdouble Tnil))
-     tdouble cc_default)) ::
+                   (mksignature (AST.Xfloat :: AST.Xfloat :: nil) AST.Xfloat
+                     cc_default)) (tdouble :: tdouble :: nil) tdouble
+     cc_default)) ::
  (___builtin_fmadd,
    Gfun(External (EF_builtin "__builtin_fmadd"
                    (mksignature
-                     (AST.Tfloat :: AST.Tfloat :: AST.Tfloat :: nil)
-                     AST.Tfloat cc_default))
-     (Tcons tdouble (Tcons tdouble (Tcons tdouble Tnil))) tdouble
-     cc_default)) ::
+                     (AST.Xfloat :: AST.Xfloat :: AST.Xfloat :: nil)
+                     AST.Xfloat cc_default))
+     (tdouble :: tdouble :: tdouble :: nil) tdouble cc_default)) ::
  (___builtin_fmsub,
    Gfun(External (EF_builtin "__builtin_fmsub"
                    (mksignature
-                     (AST.Tfloat :: AST.Tfloat :: AST.Tfloat :: nil)
-                     AST.Tfloat cc_default))
-     (Tcons tdouble (Tcons tdouble (Tcons tdouble Tnil))) tdouble
-     cc_default)) ::
+                     (AST.Xfloat :: AST.Xfloat :: AST.Xfloat :: nil)
+                     AST.Xfloat cc_default))
+     (tdouble :: tdouble :: tdouble :: nil) tdouble cc_default)) ::
  (___builtin_fnmadd,
    Gfun(External (EF_builtin "__builtin_fnmadd"
                    (mksignature
-                     (AST.Tfloat :: AST.Tfloat :: AST.Tfloat :: nil)
-                     AST.Tfloat cc_default))
-     (Tcons tdouble (Tcons tdouble (Tcons tdouble Tnil))) tdouble
-     cc_default)) ::
+                     (AST.Xfloat :: AST.Xfloat :: AST.Xfloat :: nil)
+                     AST.Xfloat cc_default))
+     (tdouble :: tdouble :: tdouble :: nil) tdouble cc_default)) ::
  (___builtin_fnmsub,
    Gfun(External (EF_builtin "__builtin_fnmsub"
                    (mksignature
-                     (AST.Tfloat :: AST.Tfloat :: AST.Tfloat :: nil)
-                     AST.Tfloat cc_default))
-     (Tcons tdouble (Tcons tdouble (Tcons tdouble Tnil))) tdouble
-     cc_default)) ::
+                     (AST.Xfloat :: AST.Xfloat :: AST.Xfloat :: nil)
+                     AST.Xfloat cc_default))
+     (tdouble :: tdouble :: tdouble :: nil) tdouble cc_default)) ::
  (___builtin_read16_reversed,
    Gfun(External (EF_builtin "__builtin_read16_reversed"
-                   (mksignature (AST.Tlong :: nil) AST.Tint16unsigned
-                     cc_default)) (Tcons (tptr tushort) Tnil) tushort
+                   (mksignature (AST.Xptr :: nil) AST.Xint16unsigned
+                     cc_default)) ((tptr tushort) :: nil) tushort
      cc_default)) ::
  (___builtin_read32_reversed,
    Gfun(External (EF_builtin "__builtin_read32_reversed"
-                   (mksignature (AST.Tlong :: nil) AST.Tint cc_default))
-     (Tcons (tptr tuint) Tnil) tuint cc_default)) ::
+                   (mksignature (AST.Xptr :: nil) AST.Xint cc_default))
+     ((tptr tuint) :: nil) tuint cc_default)) ::
  (___builtin_write16_reversed,
    Gfun(External (EF_builtin "__builtin_write16_reversed"
-                   (mksignature (AST.Tlong :: AST.Tint :: nil) AST.Tvoid
-                     cc_default)) (Tcons (tptr tushort) (Tcons tushort Tnil))
-     tvoid cc_default)) ::
+                   (mksignature (AST.Xptr :: AST.Xint16unsigned :: nil)
+                     AST.Xvoid cc_default))
+     ((tptr tushort) :: tushort :: nil) tvoid cc_default)) ::
  (___builtin_write32_reversed,
    Gfun(External (EF_builtin "__builtin_write32_reversed"
-                   (mksignature (AST.Tlong :: AST.Tint :: nil) AST.Tvoid
-                     cc_default)) (Tcons (tptr tuint) (Tcons tuint Tnil))
-     tvoid cc_default)) ::
+                   (mksignature (AST.Xptr :: AST.Xint :: nil) AST.Xvoid
+                     cc_default)) ((tptr tuint) :: tuint :: nil) tvoid
+     cc_default)) ::
  (___builtin_debug,
    Gfun(External (EF_external "__builtin_debug"
-                   (mksignature (AST.Tint :: nil) AST.Tvoid
+                   (mksignature (AST.Xint :: nil) AST.Xvoid
                      {|cc_vararg:=(Some 1); cc_unproto:=false; cc_structret:=false|}))
-     (Tcons tint Tnil) tvoid
+     (tint :: nil) tvoid
      {|cc_vararg:=(Some 1); cc_unproto:=false; cc_structret:=false|})) ::
- (___getreent,
-   Gfun(External (EF_external "__getreent"
-                   (mksignature nil AST.Tlong cc_default)) Tnil
-     (tptr (Tstruct __reent noattr)) cc_default)) ::
+ (_stdout, Gvar v_stdout) ::
  (_fprintf,
    Gfun(External (EF_external "fprintf"
-                   (mksignature (AST.Tlong :: AST.Tlong :: nil) AST.Tint
+                   (mksignature (AST.Xptr :: AST.Xptr :: nil) AST.Xint
                      {|cc_vararg:=(Some 2); cc_unproto:=false; cc_structret:=false|}))
-     (Tcons (tptr (Tstruct ___sFILE64 noattr)) (Tcons (tptr tschar) Tnil))
-     tint {|cc_vararg:=(Some 2); cc_unproto:=false; cc_structret:=false|})) ::
+     ((tptr (Tstruct __IO_FILE noattr)) :: (tptr tschar) :: nil) tint
+     {|cc_vararg:=(Some 2); cc_unproto:=false; cc_structret:=false|})) ::
  (_printf,
    Gfun(External (EF_external "printf"
-                   (mksignature (AST.Tlong :: nil) AST.Tint
+                   (mksignature (AST.Xptr :: nil) AST.Xint
                      {|cc_vararg:=(Some 1); cc_unproto:=false; cc_structret:=false|}))
-     (Tcons (tptr tschar) Tnil) tint
+     ((tptr tschar) :: nil) tint
      {|cc_vararg:=(Some 1); cc_unproto:=false; cc_structret:=false|})) ::
  (_main, Gfun(Internal f_main)) :: nil).
 
 Definition public_idents : list ident :=
-(_main :: _printf :: _fprintf :: ___getreent :: ___builtin_debug ::
+(_main :: _printf :: _fprintf :: _stdout :: ___builtin_debug ::
  ___builtin_write32_reversed :: ___builtin_write16_reversed ::
  ___builtin_read32_reversed :: ___builtin_read16_reversed ::
  ___builtin_fnmsub :: ___builtin_fnmadd :: ___builtin_fmsub ::
@@ -713,13 +641,14 @@ Definition public_idents : list ident :=
  ___builtin_ctzll :: ___builtin_ctzl :: ___builtin_ctz :: ___builtin_clzll ::
  ___builtin_clzl :: ___builtin_clz :: ___builtin_bswap16 ::
  ___builtin_bswap32 :: ___builtin_bswap :: ___builtin_bswap64 ::
- ___compcert_i64_umulh :: ___compcert_i64_smulh :: ___compcert_i64_sar ::
- ___compcert_i64_shr :: ___compcert_i64_shl :: ___compcert_i64_umod ::
- ___compcert_i64_smod :: ___compcert_i64_udiv :: ___compcert_i64_sdiv ::
- ___compcert_i64_utof :: ___compcert_i64_stof :: ___compcert_i64_utod ::
- ___compcert_i64_stod :: ___compcert_i64_dtou :: ___compcert_i64_dtos ::
- ___compcert_va_composite :: ___compcert_va_float64 ::
- ___compcert_va_int64 :: ___compcert_va_int32 :: nil).
+ ___builtin_ais_annot :: ___compcert_i64_umulh :: ___compcert_i64_smulh ::
+ ___compcert_i64_sar :: ___compcert_i64_shr :: ___compcert_i64_shl ::
+ ___compcert_i64_umod :: ___compcert_i64_smod :: ___compcert_i64_udiv ::
+ ___compcert_i64_sdiv :: ___compcert_i64_utof :: ___compcert_i64_stof ::
+ ___compcert_i64_utod :: ___compcert_i64_stod :: ___compcert_i64_dtou ::
+ ___compcert_i64_dtos :: ___compcert_va_composite ::
+ ___compcert_va_float64 :: ___compcert_va_int64 :: ___compcert_va_int32 ::
+ nil).
 
 Definition prog : Clight.program := 
   mkprogram composites global_definitions public_idents _main Logic.I.
