veric/tcb.v
@@ -17,14 +17,14 @@ Theorem VST_sound:
   forall (CS: compspecs) `(!VSTGpreS unit Σ)
      (prog: Clight.program) (initial_oracle: unit)
      (V : mpred.varspecs) (G : mpred.funspecs) (m: mem),
-     (forall `{semax.VSTGS unit Σ}, semax_prog extspec prog initial_oracle V G) ->
+     (forall `{lifting.VSTGS unit Σ}, semax_prog extspec prog initial_oracle V G) ->
      Genv.init_mem prog = Some m ->
      exists b, exists q, exists m',
        Genv.find_symbol (Genv.globalenv prog) (prog_main prog) = Some b /\
        semantics.initial_core  (Clight_core.cl_core_sem (Clight.globalenv prog))
            0 m q m' (Vptr b Ptrofs.zero) nil /\
        forall n,
-        @dry_safeN _ _ _ unit (semax.genv_symb_injective)
+        @dry_safeN _ _ _ unit (lifting.genv_symb_injective)
           (Clight_core.cl_core_sem (Clight.globalenv prog)) extspec
            (Clight.genv_genv 
             (Clight.Build_genv (Genv.globalenv prog) (Ctypes.prog_comp_env prog)) )
